theories/monotone.v
@@ -33,16 +33,6 @@ Section monotone.
         eauto. }
       specialize (Hrelated _ Permanent y Hstate Hy).
       apply std_rel_pub_rtc_Permanent in Hrelated; subst; auto.
-    - destruct Hrelated as [ [Hdom_sta Hrelated] _]. simpl in *.
-      assert (is_Some (W'.1 !! a)) as [y Hy].
-      { rewrite -elem_of_dom. apply elem_of_subseteq in Hdom_sta. apply Hdom_sta. rewrite elem_of_dom.
-        destruct Hstate; eauto. }
-      destruct Hstate as [Hmono | Hperm].
-      + left. specialize (Hrelated _ Monotemporary y Hmono Hy).
-        apply std_rel_pub_rtc_Monotemporary in Hrelated; subst;auto.
-      + right.
-        specialize (Hrelated _ Permanent y Hperm Hy).
-        apply std_rel_pub_rtc_Permanent in Hrelated; subst; auto.
   Qed.
 
   Lemma region_state_nwl_monotone_a W W' (a a' : Addr) l :
@@ -68,20 +58,6 @@ Section monotone.
       eapply rtc_implies in Hrelated.
       apply std_rel_pub_plus_rtc_Permanent in Hrelated; subst; auto.
       intros r q. destruct (decide (a' <= a)%a);auto.
-    - destruct Hrelated as [ [Hdom_sta Hrelated] _]. simpl in *.
-      assert (is_Some (W'.1 !! a)) as [y Hy].
-      { rewrite -elem_of_dom. apply elem_of_subseteq in Hdom_sta. apply Hdom_sta. rewrite elem_of_dom.
-        destruct Hstate; eauto. }
-      destruct Hstate as [Hmono | Hperm].
-      + specialize (Hrelated _ Monotemporary y Hmono Hy).
-        eapply rtc_implies in Hrelated.
-        apply std_rel_pub_rtc_Monotemporary in Hrelated; subst;auto.
-        intros r q. rewrite decide_False;auto. solve_addr.
-      + right.
-        specialize (Hrelated _ Permanent y Hperm Hy).
-        eapply rtc_implies in Hrelated.
-        apply std_rel_pub_rtc_Permanent in Hrelated; subst; auto.
-        intros r q. rewrite decide_False;auto. solve_addr.
   Qed.
 
   Lemma region_state_nwl_monotone_nm W W' a :
@@ -112,9 +88,9 @@ Section monotone.
 
   Lemma region_state_pwl_monotone_mono W W' a :
     related_sts_pub_world W W' →
-    region_state_pwl_mono W a -> region_state_pwl_mono W' a.
+    region_state_pwl W a -> region_state_pwl W' a.
   Proof.
-    rewrite /region_state_pwl_mono /std.
+    rewrite /region_state_pwl /std.
     intros Hrelated Hstate.
     destruct Hrelated as [ [Hdom_sta Hrelated ] _]. simpl in *.
     assert (is_Some (W'.1 !! a)) as [y Hy].
@@ -126,9 +102,9 @@ Section monotone.
   Lemma region_state_pwl_monotone_a W W' a a' :
     (a < a')%a →
     related_sts_a_world W W' a' →
-    region_state_pwl_mono W a -> region_state_pwl_mono W' a.
+    region_state_pwl W a -> region_state_pwl W' a.
   Proof.
-    rewrite /region_state_pwl_mono /std.
+    rewrite /region_state_pwl /std.
     intros Hle Hrelated Hstate.
     destruct Hrelated as [ [Hdom_sta Hrelated ] _]. simpl in *.
     assert (is_Some (W'.1 !! a)) as [y Hy].
@@ -139,124 +115,124 @@ Section monotone.
     intros r q. rewrite decide_False;auto. solve_addr.
   Qed.
 
-  Lemma region_state_nwl_future W W' l l' p a a':
-    (a < a')%a →
-    LocalityFlowsTo l' l ->
-    (if pwlU p then l = Directed else True) ->
-    (@future_world Σ l' a' W W') -∗
-    ⌜if pwlU p then region_state_pwl_mono W a else region_state_nwl W a l⌝ -∗
-                                                   ⌜region_state_nwl W' a l'⌝.
-  Proof.
-    intros Hlt Hlflows Hloc. iIntros "Hfuture %".
-    destruct l'; simpl; iDestruct "Hfuture" as %Hf; iPureIntro.
-    - assert (l = Global) as -> by (destruct l; simpl in Hlflows; tauto).
-      destruct (pwlU p) eqn:HpwlU; try congruence.
-      eapply region_state_nwl_monotone_nm_nl; eauto.
-    - destruct (pwlU p).
-      + subst l. inversion Hlflows.
-      + eapply region_state_nwl_monotone_nm_nl; eauto.
-        destruct l;inversion Hlflows;auto.
-    - destruct (pwlU p).
-      + subst l. simpl in *.
-        left. eapply region_state_pwl_monotone_a;eauto.
-      + destruct l.
-        * right. eapply region_state_nwl_monotone_nm_nl;eauto.
-          apply related_sts_pub_plus_priv_world.
-          eapply related_sts_a_pub_plus_world;eauto.
-        * right. eapply region_state_nwl_monotone_nm_nl;eauto.
-          apply related_sts_pub_plus_priv_world.
-          eapply related_sts_a_pub_plus_world;eauto.
-        * destruct H0 as [a0 | a0].
-          left. eapply region_state_pwl_monotone_a;eauto.
-          right. eapply region_state_nwl_monotone_nm_nl;eauto.
-          apply related_sts_pub_plus_priv_world.
-          eapply related_sts_a_pub_plus_world;eauto.
-  Qed.
+  (* Lemma region_state_nwl_future W W' l l' p a a': *)
+  (*   (a < a')%a → *)
+  (*   LocalityFlowsTo l' l -> *)
+  (*   (if pwlU p then l = Directed else True) -> *)
+  (*   (@future_world Σ l' a' W W') -∗ *)
+  (*   ⌜if pwlU p then region_state_pwl_mono W a else region_state_nwl W a l⌝ -∗ *)
+  (*                                                  ⌜region_state_nwl W' a l'⌝. *)
+  (* Proof. *)
+  (*   intros Hlt Hlflows Hloc. iIntros "Hfuture %". *)
+  (*   destruct l'; simpl; iDestruct "Hfuture" as %Hf; iPureIntro. *)
+  (*   - assert (l = Global) as -> by (destruct l; simpl in Hlflows; tauto). *)
+  (*     destruct (pwlU p) eqn:HpwlU; try congruence. *)
+  (*     eapply region_state_nwl_monotone_nm_nl; eauto. *)
+  (*   - destruct (pwlU p). *)
+  (*     + subst l. inversion Hlflows. *)
+  (*     + eapply region_state_nwl_monotone_nm_nl; eauto. *)
+  (*       destruct l;inversion Hlflows;auto. *)
+  (*   - destruct (pwlU p). *)
+  (*     + subst l. simpl in *. *)
+  (*       left. eapply region_state_pwl_monotone_a;eauto. *)
+  (*     + destruct l. *)
+  (*       * right. eapply region_state_nwl_monotone_nm_nl;eauto. *)
+  (*         apply related_sts_pub_plus_priv_world. *)
+  (*         eapply related_sts_a_pub_plus_world;eauto. *)
+  (*       * right. eapply region_state_nwl_monotone_nm_nl;eauto. *)
+  (*         apply related_sts_pub_plus_priv_world. *)
+  (*         eapply related_sts_a_pub_plus_world;eauto. *)
+  (*       * destruct H0 as [a0 | a0]. *)
+  (*         left. eapply region_state_pwl_monotone_a;eauto. *)
+  (*         right. eapply region_state_nwl_monotone_nm_nl;eauto. *)
+  (*         apply related_sts_pub_plus_priv_world. *)
+  (*         eapply related_sts_a_pub_plus_world;eauto. *)
+  (* Qed. *)
 
-  Lemma region_state_U_monotone W W' a :
-    related_sts_priv_world W W' →
-    region_state_U W a -> region_state_U W' a.
-  Proof.
-    rewrite /region_state_U /std.
-    intros Hrelated Hstate.
-    destruct Hrelated as [ [Hdom_sta Hrelated ] _]. simpl in *.
-    assert (is_Some (W'.1 !! a)) as [y Hy].
-    { rewrite -elem_of_dom. apply elem_of_subseteq in Hdom_sta. apply Hdom_sta. rewrite elem_of_dom;eauto. }
-    specialize (Hrelated _ Permanent y Hstate Hy).
-    apply std_rel_rtc_Permanent in Hrelated; auto. subst y; auto.
-  Qed.
+  (* Lemma region_state_U_monotone W W' a : *)
+  (*   related_sts_priv_world W W' → *)
+  (*   region_state_U W a -> region_state_U W' a. *)
+  (* Proof. *)
+  (*   rewrite /region_state_U /std. *)
+  (*   intros Hrelated Hstate. *)
+  (*   destruct Hrelated as [ [Hdom_sta Hrelated ] _]. simpl in *. *)
+  (*   assert (is_Some (W'.1 !! a)) as [y Hy]. *)
+  (*   { rewrite -elem_of_dom. apply elem_of_subseteq in Hdom_sta. apply Hdom_sta. rewrite elem_of_dom;eauto. } *)
+  (*   specialize (Hrelated _ Permanent y Hstate Hy). *)
+  (*   apply std_rel_rtc_Permanent in Hrelated; auto. subst y; auto. *)
+  (* Qed. *)
 
-  Lemma region_state_U_monotone_mono W W' a :
-    related_sts_pub_plus_world W W' →
-    region_state_U_mono W a -> region_state_U_mono W' a.
-  Proof.
-    rewrite /region_state_U_mono /std.
-    intros Hrelated Hstate.
-    destruct Hrelated as [ [Hdom_sta Hrelated ] _]. simpl in *.
-    assert (is_Some (W'.1 !! a)) as [y Hy].
-    { rewrite -elem_of_dom. apply elem_of_subseteq in Hdom_sta. apply Hdom_sta. rewrite elem_of_dom;eauto.
-      destruct Hstate as [Hstate | [Hstate | [w Hstate] ] ];eauto. }
-    destruct Hstate as [Hstate | [Hstate | [w Hstate] ] ].
-    - specialize (Hrelated _ _ y Hstate Hy).
-      apply std_rel_pub_plus_rtc_Monotemporary in Hrelated;eauto.
-      destruct Hrelated as [-> | [? ->] ];subst;rewrite Hy;eauto.
-    - specialize (Hrelated _ Permanent y Hstate Hy).
-      apply std_rel_pub_plus_rtc_Permanent in Hrelated; auto. subst y; auto.
-    - specialize (Hrelated _ _ y Hstate Hy).
-      eapply std_rel_pub_plus_rtc_Uninitialized in Hrelated; eauto.
-      destruct Hrelated as [-> | [? ->] ]; eauto.
-  Qed.
+  (* Lemma region_state_U_monotone_mono W W' a : *)
+  (*   related_sts_pub_plus_world W W' → *)
+  (*   region_state_U_mono W a -> region_state_U_mono W' a. *)
+  (* Proof. *)
+  (*   rewrite /region_state_U_mono /std. *)
+  (*   intros Hrelated Hstate. *)
+  (*   destruct Hrelated as [ [Hdom_sta Hrelated ] _]. simpl in *. *)
+  (*   assert (is_Some (W'.1 !! a)) as [y Hy]. *)
+  (*   { rewrite -elem_of_dom. apply elem_of_subseteq in Hdom_sta. apply Hdom_sta. rewrite elem_of_dom;eauto. *)
+  (*     destruct Hstate as [Hstate | [Hstate | [w Hstate] ] ];eauto. } *)
+  (*   destruct Hstate as [Hstate | [Hstate | [w Hstate] ] ]. *)
+  (*   - specialize (Hrelated _ _ y Hstate Hy). *)
+  (*     apply std_rel_pub_plus_rtc_Monotemporary in Hrelated;eauto. *)
+  (*     destruct Hrelated as [-> | [? ->] ];subst;rewrite Hy;eauto. *)
+  (*   - specialize (Hrelated _ Permanent y Hstate Hy). *)
+  (*     apply std_rel_pub_plus_rtc_Permanent in Hrelated; auto. subst y; auto. *)
+  (*   - specialize (Hrelated _ _ y Hstate Hy). *)
+  (*     eapply std_rel_pub_plus_rtc_Uninitialized in Hrelated; eauto. *)
+  (*     destruct Hrelated as [-> | [? ->] ]; eauto. *)
+  (* Qed. *)
 
-  Lemma region_state_U_pwl_monotone_mono W W' a :
-    related_sts_pub_world W W' →
-    region_state_U_pwl_mono W a -> region_state_U_pwl_mono W' a.
-  Proof.
-    rewrite /region_state_U /std.
-    intros Hrelated Hstate.
-    destruct Hrelated as [ [Hdom_sta Hrelated ] _]. simpl in *.
-    assert (is_Some (W'.1 !! a)) as [y Hy].
-    { rewrite -elem_of_dom. apply elem_of_subseteq in Hdom_sta. apply Hdom_sta. rewrite elem_of_dom;eauto.
-      destruct Hstate as [? | [? ?] ]; eauto. }
-    destruct Hstate as [Hstate|[? Hstate] ].
-    - specialize (Hrelated _ Monotemporary y Hstate Hy).
-      destruct (decide (y = Monotemporary)); subst; left; auto.
-      apply std_rel_pub_rtc_Monotemporary in Hrelated; auto. contradiction.
-    - specialize (Hrelated _ (Uninitialized x) y Hstate Hy).
-      eapply std_rel_pub_rtc_Uninitialized in Hrelated; eauto. destruct Hrelated;subst y; [left | right]; eauto.
-  Qed.
+  (* Lemma region_state_U_pwl_monotone_mono W W' a : *)
+  (*   related_sts_pub_world W W' → *)
+  (*   region_state_U_pwl_mono W a -> region_state_U_pwl_mono W' a. *)
+  (* Proof. *)
+  (*   rewrite /region_state_U /std. *)
+  (*   intros Hrelated Hstate. *)
+  (*   destruct Hrelated as [ [Hdom_sta Hrelated ] _]. simpl in *. *)
+  (*   assert (is_Some (W'.1 !! a)) as [y Hy]. *)
+  (*   { rewrite -elem_of_dom. apply elem_of_subseteq in Hdom_sta. apply Hdom_sta. rewrite elem_of_dom;eauto. *)
+  (*     destruct Hstate as [? | [? ?] ]; eauto. } *)
+  (*   destruct Hstate as [Hstate|[? Hstate] ]. *)
+  (*   - specialize (Hrelated _ Monotemporary y Hstate Hy). *)
+  (*     destruct (decide (y = Monotemporary)); subst; left; auto. *)
+  (*     apply std_rel_pub_rtc_Monotemporary in Hrelated; auto. contradiction. *)
+  (*   - specialize (Hrelated _ (Uninitialized x) y Hstate Hy). *)
+  (*     eapply std_rel_pub_rtc_Uninitialized in Hrelated; eauto. destruct Hrelated;subst y; [left | right]; eauto. *)
+  (* Qed. *)
 
-  Lemma region_state_U_pwl_monotone_mono_a W W' a a' :
-    related_sts_a_world W W' a' →
-    region_state_U_pwl_mono W a -> region_state_U_pwl_mono W' a.
-  Proof.
-    rewrite /region_state_U /std.
-    intros Hrelated Hstate.
-    destruct Hrelated as [ [Hdom_sta Hrelated ] _]. simpl in *.
-    assert (is_Some (W'.1 !! a)) as [y Hy].
-    { rewrite -elem_of_dom. apply elem_of_subseteq in Hdom_sta. apply Hdom_sta. rewrite elem_of_dom;eauto.
-      destruct Hstate as [? | [? ?] ]; eauto. }
-    destruct Hstate as [Hstate|[? Hstate] ].
-    - specialize (Hrelated _ Monotemporary y Hstate Hy).
-      destruct (decide (y = Monotemporary)); subst; auto. left;auto.
-      destruct (decide (a' <= a)%a).
-      + apply std_rel_pub_plus_rtc_Monotemporary in Hrelated; subst;auto.
-        destruct Hrelated as [-> | [? ->] ];
-          rewrite /region_state_U_pwl_mono;eauto.
-      + apply std_rel_pub_rtc_Monotemporary in Hrelated; subst;auto. contradiction.
-    - specialize (Hrelated _ (Uninitialized x) y Hstate Hy).
-      destruct (decide (a' <= a)%a).
-      + eapply std_rel_pub_plus_rtc_Uninitialized in Hrelated; eauto.
-        destruct Hrelated as [Hy' | [w' Hy'] ]; subst y; [left | right]; eauto.
-      + eapply std_rel_pub_rtc_Uninitialized in Hrelated; eauto.
-        destruct Hrelated; subst y; [left | right]; eauto.
-  Qed.
+  (* Lemma region_state_U_pwl_monotone_mono_a W W' a a' : *)
+  (*   related_sts_a_world W W' a' → *)
+  (*   region_state_U_pwl_mono W a -> region_state_U_pwl_mono W' a. *)
+  (* Proof. *)
+  (*   rewrite /region_state_U /std. *)
+  (*   intros Hrelated Hstate. *)
+  (*   destruct Hrelated as [ [Hdom_sta Hrelated ] _]. simpl in *. *)
+  (*   assert (is_Some (W'.1 !! a)) as [y Hy]. *)
+  (*   { rewrite -elem_of_dom. apply elem_of_subseteq in Hdom_sta. apply Hdom_sta. rewrite elem_of_dom;eauto. *)
+  (*     destruct Hstate as [? | [? ?] ]; eauto. } *)
+  (*   destruct Hstate as [Hstate|[? Hstate] ]. *)
+  (*   - specialize (Hrelated _ Monotemporary y Hstate Hy). *)
+  (*     destruct (decide (y = Monotemporary)); subst; auto. left;auto. *)
+  (*     destruct (decide (a' <= a)%a). *)
+  (*     + apply std_rel_pub_plus_rtc_Monotemporary in Hrelated; subst;auto. *)
+  (*       destruct Hrelated as [-> | [? ->] ]; *)
+  (*         rewrite /region_state_U_pwl_mono;eauto. *)
+  (*     + apply std_rel_pub_rtc_Monotemporary in Hrelated; subst;auto. contradiction. *)
+  (*   - specialize (Hrelated _ (Uninitialized x) y Hstate Hy). *)
+  (*     destruct (decide (a' <= a)%a). *)
+  (*     + eapply std_rel_pub_plus_rtc_Uninitialized in Hrelated; eauto. *)
+  (*       destruct Hrelated as [Hy' | [w' Hy'] ]; subst y; [left | right]; eauto. *)
+  (*     + eapply std_rel_pub_rtc_Uninitialized in Hrelated; eauto. *)
+  (*       destruct Hrelated; subst y; [left | right]; eauto. *)
+  (* Qed. *)
 
   (* The following lemma is not required for monotonicity, but is interesting for use in examples *)
   Lemma region_state_U_pwl_monotone_same W W' g a :
     related_sts_pub_world W W' →
     (std W) !! a = Some (Monostatic g) -> (std W') !! a = Some (Monostatic g).
   Proof.
-    rewrite /region_state_U /std.
+    rewrite /std.
     intros Hrelated Hstate.
     destruct Hrelated as [ [Hdom_sta Hrelated ] _]. simpl in *.
     assert (is_Some (W'.1 !! a)) as [y Hy].
@@ -272,7 +248,7 @@ Section monotone.
     (std W') !! a = Some Monotemporary ∨
     (std W') !! a = Some Permanent.
   Proof.
-    rewrite /region_state_pwl_mono /std.
+    rewrite /region_state_pwl /std.
     intros Hrelated Hstate.
     destruct Hrelated as [ [Hdom_sta Hrelated ] _]. simpl in *.
     assert (is_Some (W'.1 !! a)) as [y Hy].
@@ -305,11 +281,8 @@ Section monotone.
     - destruct l; auto.
       iApply (big_sepL_mono with "Hw").
       iIntros (n y Hsome) "Hw".
-      iDestruct "Hw" as "#[Hrw Hrel]".
-      iSplit;eauto. iFrame "#".
-      iDestruct "Hrel" as %Hrel.
-      iPureIntro.
-      apply region_state_pwl_monotone_mono with W;auto.
+      iDestruct "Hw" as (p) "(%Hflow & Hrw & %Hrel)".
+      eapply region_state_pwl_monotone_mono in Hrel;auto.
     - iApply (big_sepL_mono with "Hw").
       iIntros (n y Hsome) "Hw".
       iDestruct "Hw" as (P Hpers) "#[Hrw Hrel]".
@@ -319,18 +292,13 @@ Section monotone.
     - iModIntro. iIntros (r W'').
       destruct l; simpl.
       + iIntros (Hrelated').
-        iAssert (future_world Global a W W'')%I as "Hrelated".
+        iAssert (future_world Global W W'')%I as "Hrelated".
         { iPureIntro. apply related_sts_pub_priv_trans_world with W'; auto. }
         iSpecialize ("Hw" $! r W'' with "Hrelated").
         iApply "Hw".
       + iIntros (Hrelated').
-        iAssert (future_world Local a W W'')%I as "Hrelated".
+        iAssert (future_world Local W W'')%I as "Hrelated".
         { iPureIntro. apply related_sts_pub_priv_trans_world with W'; auto. }
-        iSpecialize ("Hw" $! r W'' with "Hrelated").
-        iApply "Hw".
-      + iIntros (Hrelated').
-        iAssert (future_world Directed a0 W W'')%I as "Hrelated".
-        { iPureIntro. apply related_sts_pub_a_trans_world with W'; auto. }
         iSpecialize ("Hw" $! r W'' with "Hrelated").
         iApply "Hw".
     - iApply (big_sepL_mono with "Hw").
@@ -342,125 +310,15 @@ Section monotone.
     - destruct l; auto.
       iApply (big_sepL_mono with "Hw").
       iIntros (n y Hsome) "Hw".
-      iDestruct "Hw" as "#[Hrw Hrel]".
-      iSplit;eauto. iFrame "#".
-      iDestruct "Hrel" as %Hrel.
-      iPureIntro. apply region_state_pwl_monotone_mono with W;auto.
-    - destruct l; simpl.
-      + iApply (big_sepL_mono with "Hw").
-        iIntros (n y Hsome) "Hw".
-        iDestruct "Hw" as "#[Hrw Hst]".
-        iSplit;eauto. iFrame "#".
-        iDestruct "Hst" as %Hst.
-        iPureIntro. eapply (region_state_nwl_monotone W W' _ Global); auto.
-      + iDestruct "Hw" as "[Hw1 Hw2]".
-        iSplitL "Hw1".
-        * iApply (big_sepL_mono with "Hw1").
-          iIntros (n y Hsome) "Hw".
-          iDestruct "Hw" as "#[Hrw Hst ]".
-          iSplit;eauto. iFrame "#".
-          iDestruct "Hst" as %Hstd.
-          iPureIntro. eapply (region_state_nwl_monotone W W' _ Local); auto.
-        * iApply (big_sepL_mono with "Hw2").
-          iIntros (n y Hsome) "Hw".
-          iDestruct "Hw" as "#[Hrw Hst ]".
-          iSplit;eauto. iFrame "#".
-          iDestruct "Hst" as %Hst.
-          iPureIntro.
-          eapply region_state_U_monotone; eauto.
-          apply related_sts_pub_priv_world;auto.
-      + iDestruct "Hw" as "[Hw1 Hw2]".
-        iSplitL "Hw1".
-        * iApply (big_sepL_mono with "Hw1").
-          iIntros (n y Hsome) "Hw".
-          iDestruct "Hw" as "#[Hrw Hst ]".
-          iSplit;eauto. iFrame "#".
-          iDestruct "Hst" as %Hstd.
-          iPureIntro. eapply (region_state_nwl_monotone W W' _ Directed); auto.
-        * iApply (big_sepL_mono with "Hw2").
-          iIntros (n y Hsome) "Hw".
-          iDestruct "Hw" as "#[Hrw Hst ]".
-          iSplit;eauto. iFrame "#".
-          iDestruct "Hst" as %Hst.
-          iPureIntro.
-          eapply region_state_U_monotone_mono; eauto.
-          apply related_sts_pub_pub_plus_world;auto.
-    - destruct l; auto.
-      iDestruct "Hw" as "[Hbe Hexec]".
-      iSplit.
-      { iApply (big_sepL_mono with "Hbe").
-        iIntros (n y Hsome) "Hw".
-        iDestruct "Hw" as "#[Hrw Hrel ]".
-        iSplit;eauto. iFrame "#".
-        iDestruct "Hrel" as %Hrel.
-        iPureIntro. apply region_state_pwl_monotone_mono with W;auto. }
-      { iApply (big_sepL_mono with "Hexec").
-        iIntros (n y Hsome) "Hw".
-        iDestruct "Hw" as "#[Hrw Hrel ]".
-        iSplit;eauto. iFrame "#".
-        iDestruct "Hrel" as %Hrel.
-        iPureIntro. apply region_state_U_pwl_monotone_mono with W;auto. }
-    - destruct l; simpl.
-      + iApply (big_sepL_mono with "Hw").
-        iIntros (n y Hsome) "Hw".
-        iDestruct "Hw" as "#[Hrw Hst ]".
-        iSplit;eauto. iFrame "#".
-        iDestruct "Hst" as %Hst.
-        iPureIntro. eapply (region_state_nwl_monotone W W' _ Global); auto.
-      + iDestruct "Hw" as "[Hw1 Hw2]".
-        iSplitL "Hw1".
-        * iApply (big_sepL_mono with "Hw1").
-          iIntros (n y Hsome) "Hw".
-          iDestruct "Hw" as "#[Hrw Hst ]".
-          iSplit;eauto. iFrame "#".
-          iDestruct "Hst" as %Hstd.
-          iPureIntro. eapply (region_state_nwl_monotone W W' _ Local); auto.
-        * iApply (big_sepL_mono with "Hw2").
-          iIntros (n y Hsome) "Hw".
-          iDestruct "Hw" as "#[Hrw Hst ]".
-          iSplit;eauto. iFrame "#".
-          iDestruct "Hst" as %Hst.
-          iPureIntro.
-          eapply region_state_U_monotone; eauto.
-          apply related_sts_pub_priv_world;auto.
-      + iDestruct "Hw" as "[Hw1 Hw2]".
-        iSplitL "Hw1".
-        * iApply (big_sepL_mono with "Hw1").
-          iIntros (n y Hsome) "Hw".
-          iDestruct "Hw" as "#[Hrw Hst ]".
-          iSplit;eauto. iFrame "#".
-          iDestruct "Hst" as %Hstd.
-          iPureIntro. eapply (region_state_nwl_monotone W W' _ Directed); auto.
-        * iApply (big_sepL_mono with "Hw2").
-          iIntros (n y Hsome) "Hw".
-          iDestruct "Hw" as "#[Hrw Hst ]".
-          iSplit;eauto. iFrame "#".
-          iDestruct "Hst" as %Hst.
-          iPureIntro.
-          eapply region_state_U_monotone_mono; eauto.
-          apply related_sts_pub_pub_plus_world;auto.
-    - destruct l; auto.
-      iDestruct "Hw" as "[Hbe Hexec]".
-      iSplit.
-      { iApply (big_sepL_mono with "Hbe").
-        iIntros (n y Hsome) "Hw".
-        iDestruct "Hw" as "#[Hrw Hrel ]".
-        iSplit;eauto. iFrame "#".
-        iDestruct "Hrel" as %Hrel.
-        iPureIntro. apply region_state_pwl_monotone_mono with W;auto. }
-      { iApply (big_sepL_mono with "Hexec").
-        iIntros (n y Hsome) "Hw".
-        iDestruct "Hw" as "#[Hrw Hrel ]".
-        iSplit;eauto. iFrame "#".
-        iDestruct "Hrel" as %Hrel.
-        iPureIntro. apply region_state_U_pwl_monotone_mono with W;auto. }
+      iDestruct "Hw" as (p) "(%Hflow & Hrw & %Hrel)".
+      eapply region_state_pwl_monotone_mono in Hrel;auto.
   Qed.
 
-  Definition aOf (w : Word) : Addr :=
-    match w with
-    | inl _ => addr_reg.top
-    | inr (p,_,_,e,a) => if isU p then a else e
-    end.
+  (* Definition aOf (w : Word) : Addr := *)
+  (*   match w with *)
+  (*   | inl _ => addr_reg.top *)
+  (*   | inr (p,_,_,e,a) => if isU p then a else e *)
+  (*   end. *)
 
   Lemma region_addrs_lookup_le b e a n :
     region_addrs b e !! n = Some a →
@@ -473,306 +331,311 @@ Section monotone.
     solve_addr.
   Qed.
 
-  Lemma interp_monotone_a W W' w :
-    ⌜related_sts_a_world W W' (aOf w)⌝ -∗
-    interp W w -∗ interp W' w.
-  Proof.
-    iIntros (Hrelated) "#Hw".
-    rewrite /interp /= fixpoint_interp1_eq /=.
-    destruct w; rewrite fixpoint_interp1_eq /=; auto.
-    destruct c,p,p,p,p; auto; simpl in Hrelated.
-    - iApply (big_sepL_mono with "Hw").
-      iIntros (n y Hsome) "Hw".
-      iDestruct "Hw" as (P Hpers) "#[Hrw Hrel]".
-      iExists _. iSplit;eauto. iFrame "#".
-      iDestruct "Hrel" as %Hrel.
-      iPureIntro. apply region_state_nwl_monotone_a with W a0;auto.
-      eapply region_addrs_lookup_le;eauto.
-    - iApply (big_sepL_mono with "Hw").
-      iIntros (n y Hsome) "Hw".
-      iDestruct "Hw" as "#[Hrw Hrel]".
-      iSplit;eauto. iFrame "#".
-      iDestruct "Hrel" as %Hrel.
-      iPureIntro. apply region_state_nwl_monotone_a with W a0;auto. eapply region_addrs_lookup_le;eauto. 
-    - destruct l; auto.
-      iApply (big_sepL_mono with "Hw").
-      iIntros (n y Hsome) "Hw".
-      iDestruct "Hw" as "#[Hrw Hrel]".
-      iSplit;eauto. iFrame "#".
-      iDestruct "Hrel" as %Hrel.
-      iPureIntro.
-      apply region_state_pwl_monotone_a with W a0;auto. eapply region_addrs_lookup_le;eauto. 
-    - iApply (big_sepL_mono with "Hw").
-      iIntros (n y Hsome) "Hw".
-      iDestruct "Hw" as (P Hpers) "#[Hrw Hrel]".
-      iExists _. iSplit;eauto. iFrame "#".
-      iDestruct "Hrel" as %Hrel.
-      iPureIntro. apply region_state_nwl_monotone_a with W a0;auto. eapply region_addrs_lookup_le;eauto. 
-    - iModIntro. iIntros (r W'').
-      destruct l; simpl.
-      + iIntros (Hrelated').
-        iAssert (future_world Global a W W'')%I as "Hrelated".
-        { iPureIntro. apply related_sts_a_priv_trans_world with W' a0; auto. }
-        iSpecialize ("Hw" $! r W'' with "Hrelated").
-        iApply "Hw".
-      + iIntros (Hrelated').
-        iAssert (future_world Local a W W'')%I as "Hrelated".
-        { iPureIntro. apply related_sts_a_priv_trans_world with W' a0; auto. }
-        iSpecialize ("Hw" $! r W'' with "Hrelated").
-        iApply "Hw".
-      + iIntros (Hrelated').
-        iAssert (future_world Directed a0 W W'')%I as "Hrelated".
-        { iPureIntro. apply related_sts_a_trans_world with W';auto. }
-        iSpecialize ("Hw" $! r W'' with "Hrelated").
-        iApply "Hw".
-    - iApply (big_sepL_mono with "Hw").
-      iIntros (n y Hsome) "Hw".
-      iDestruct "Hw" as "#[Hrw Hrel]".
-      iSplit;eauto. iFrame "#".
-      iDestruct "Hrel" as %Hrel.
-      iPureIntro. apply region_state_nwl_monotone_a with W a0;auto. eapply region_addrs_lookup_le;eauto. 
-    - destruct l; auto.
-      iApply (big_sepL_mono with "Hw").
-      iIntros (n y Hsome) "Hw".
-      iDestruct "Hw" as "#[Hrw Hrel]".
-      iSplit;eauto. iFrame "#".
-      iDestruct "Hrel" as %Hrel.
-      iPureIntro. apply region_state_pwl_monotone_a with W a0;auto. eapply region_addrs_lookup_le;eauto. 
-    - destruct l; simpl.
-      + iApply (big_sepL_mono with "Hw").
-        iIntros (n y Hsome) "Hw".
-        iDestruct "Hw" as "#[Hrw Hst]".
-        iSplit;eauto. iFrame "#".
-        iDestruct "Hst" as %Hst.
-        iPureIntro. apply region_state_nwl_monotone_nm_nl with W;auto.
-        apply related_sts_pub_plus_priv_world, related_sts_a_pub_plus_world with a;auto. 
-      + iDestruct "Hw" as "[Hw1 Hw2]".
-        iSplitL "Hw1".
-        * iApply (big_sepL_mono with "Hw1").
-          iIntros (n y Hsome) "Hw".
-          iDestruct "Hw" as "#[Hrw Hst ]".
-          iSplit;eauto. iFrame "#".
-          iDestruct "Hst" as %Hstd.
-          iPureIntro. eapply (region_state_nwl_monotone_a W W' _ (addr_reg.min a a0) Local); auto.
-          eapply region_addrs_lookup_le;eauto.  apply related_sts_a_weak_world with a;auto. solve_addr. 
-        * iApply (big_sepL_mono with "Hw2").
-          iIntros (n y Hsome) "Hw".
-          iDestruct "Hw" as "#[Hrw Hst ]".
-          iSplit;eauto. iFrame "#".
-          iDestruct "Hst" as %Hst.
-          iPureIntro.
-          eapply region_state_U_monotone; eauto.
-          apply related_sts_pub_plus_priv_world. apply related_sts_a_pub_plus_world with a;auto.
-      + iDestruct "Hw" as "[Hw1 Hw2]".
-        iSplitL "Hw1".
-        * iApply (big_sepL_mono with "Hw1").
-          iIntros (n y Hsome) "Hw".
-          iDestruct "Hw" as "#[Hrw Hst ]".
-          iSplit;eauto. iFrame "#".
-          iDestruct "Hst" as %Hstd.
-          iPureIntro. eapply (region_state_nwl_monotone_a W W' _ (addr_reg.min a a0) Directed); auto.
-          eapply region_addrs_lookup_le;eauto.  apply related_sts_a_weak_world with a;auto. solve_addr.
-        * iApply (big_sepL_mono with "Hw2").
-          iIntros (n y Hsome) "Hw".
-          iDestruct "Hw" as "#[Hrw Hst ]".
-          iSplit;eauto. iFrame "#".
-          iDestruct "Hst" as %Hst.
-          iPureIntro.
-          eapply region_state_U_monotone_mono; eauto.
-          apply related_sts_a_pub_plus_world with a;auto.
-    - destruct l; auto.
-      iDestruct "Hw" as "[Hbe Hexec]".
-      iSplit.
-      { iApply (big_sepL_mono with "Hbe").
-        iIntros (n y Hsome) "Hw".
-        iDestruct "Hw" as "#[Hrw Hrel ]".
-        iSplit;eauto. iFrame "#".
-        iDestruct "Hrel" as %Hrel.
-        iPureIntro. apply region_state_pwl_monotone_a with W (addr_reg.min a a0);auto.
-        eapply region_addrs_lookup_le;eauto. apply related_sts_a_weak_world with a;auto. solve_addr.
-      }
-      { iApply (big_sepL_mono with "Hexec").
-        iIntros (n y Hsome) "Hw".
-        iDestruct "Hw" as "#[Hrw Hrel ]".
-        iSplit;eauto. iFrame "#".
-        iDestruct "Hrel" as %Hrel.
-        iPureIntro. apply region_state_U_pwl_monotone_mono_a with W (addr_reg.min a a0);auto.
-        apply related_sts_a_weak_world with a;auto. solve_addr. }
-    - destruct l; simpl.
-      + iApply (big_sepL_mono with "Hw").
-        iIntros (n y Hsome) "Hw".
-        iDestruct "Hw" as "#[Hrw Hst ]".
-        iSplit;eauto. iFrame "#".
-        iDestruct "Hst" as %Hst.
-        iPureIntro. apply region_state_nwl_monotone_nm_nl with W;auto.
-        apply related_sts_pub_plus_priv_world, related_sts_a_pub_plus_world with a;auto.
-      + iDestruct "Hw" as "[Hw1 Hw2]".
-        iSplitL "Hw1".
-        * iApply (big_sepL_mono with "Hw1").
-          iIntros (n y Hsome) "Hw".
-          iDestruct "Hw" as "#[Hrw Hst ]".
-          iSplit;eauto. iFrame "#".
-          iDestruct "Hst" as %Hstd.
-          iPureIntro. eapply (region_state_nwl_monotone_a W W' _ (addr_reg.min a a0) Local); auto.
-          eapply region_addrs_lookup_le;eauto. apply related_sts_a_weak_world with a;auto. solve_addr.
-        * iApply (big_sepL_mono with "Hw2").
-          iIntros (n y Hsome) "Hw".
-          iDestruct "Hw" as "#[Hrw Hst ]".
-          iSplit;eauto. iFrame "#".
-          iDestruct "Hst" as %Hst.
-          iPureIntro.
-          eapply region_state_U_monotone; eauto.
-          apply related_sts_pub_plus_priv_world.
-          apply related_sts_a_pub_plus_world with a;auto.
-      + iDestruct "Hw" as "[Hw1 Hw2]".
-        iSplitL "Hw1".
-        * iApply (big_sepL_mono with "Hw1").
-          iIntros (n y Hsome) "Hw".
-          iDestruct "Hw" as "#[Hrw Hst ]".
-          iSplit;eauto. iFrame "#".
-          iDestruct "Hst" as %Hstd.
-          iPureIntro. eapply (region_state_nwl_monotone_a W W' _ (addr_reg.min a a0)  Directed); auto.
-          eapply region_addrs_lookup_le;eauto. apply related_sts_a_weak_world with a;auto. solve_addr.
-         * iApply (big_sepL_mono with "Hw2").
-          iIntros (n y Hsome) "Hw".
-          iDestruct "Hw" as "#[Hrw Hst ]".
-          iSplit;eauto. iFrame "#".
-          iDestruct "Hst" as %Hst.
-          iPureIntro.
-          eapply region_state_U_monotone_mono; eauto.
-          apply related_sts_a_pub_plus_world with a;auto.
-    - destruct l; auto.
-      iDestruct "Hw" as "[Hbe Hexec]".
-      iSplit.
-      { iApply (big_sepL_mono with "Hbe").
-        iIntros (n y Hsome) "Hw".
-        iDestruct "Hw" as "#[Hrw Hrel ]".
-        iSplit;eauto. iFrame "#".
-        iDestruct "Hrel" as %Hrel.
-        iPureIntro. apply region_state_pwl_monotone_a with W (addr_reg.min a a0);auto.
-        eapply region_addrs_lookup_le;eauto. apply related_sts_a_weak_world with a;auto. solve_addr.
-      }
-      { iApply (big_sepL_mono with "Hexec").
-        iIntros (n y Hsome) "Hw".
-        iDestruct "Hw" as "#[Hrw Hrel ]".
-        iSplit;eauto. iFrame "#".
-        iDestruct "Hrel" as %Hrel.
-        iPureIntro. apply region_state_U_pwl_monotone_mono_a with W a;auto. }
-  Qed.
+  (* Lemma interp_monotone_a W W' w : *)
+  (*   ⌜related_sts_a_world W W' (aOf w)⌝ -∗ *)
+  (*   interp W w -∗ interp W' w. *)
+  (* Proof. *)
+  (*   iIntros (Hrelated) "#Hw". *)
+  (*   rewrite /interp /= fixpoint_interp1_eq /=. *)
+  (*   destruct w; rewrite fixpoint_interp1_eq /=; auto. *)
+  (*   destruct c,p,p,p,p; auto; simpl in Hrelated. *)
+  (*   - iApply (big_sepL_mono with "Hw"). *)
+  (*     iIntros (n y Hsome) "Hw". *)
+  (*     iDestruct "Hw" as (P Hpers) "#[Hrw Hrel]". *)
+  (*     iExists _. iSplit;eauto. iFrame "#". *)
+  (*     iDestruct "Hrel" as %Hrel. *)
+  (*     iPureIntro. apply region_state_nwl_monotone_a with W a0;auto. *)
+  (*     eapply region_addrs_lookup_le;eauto. *)
+  (*   - iApply (big_sepL_mono with "Hw"). *)
+  (*     iIntros (n y Hsome) "Hw". *)
+  (*     iDestruct "Hw" as "#[Hrw Hrel]". *)
+  (*     iSplit;eauto. iFrame "#". *)
+  (*     iDestruct "Hrel" as %Hrel. *)
+  (*     iPureIntro. apply region_state_nwl_monotone_a with W a0;auto. eapply region_addrs_lookup_le;eauto.  *)
+  (*   - destruct l; auto. *)
+  (*     iApply (big_sepL_mono with "Hw"). *)
+  (*     iIntros (n y Hsome) "Hw". *)
+  (*     iDestruct "Hw" as "#[Hrw Hrel]". *)
+  (*     iSplit;eauto. iFrame "#". *)
+  (*     iDestruct "Hrel" as %Hrel. *)
+  (*     iPureIntro. *)
+  (*     apply region_state_pwl_monotone_a with W a0;auto. eapply region_addrs_lookup_le;eauto.  *)
+  (*   - iApply (big_sepL_mono with "Hw"). *)
+  (*     iIntros (n y Hsome) "Hw". *)
+  (*     iDestruct "Hw" as (P Hpers) "#[Hrw Hrel]". *)
+  (*     iExists _. iSplit;eauto. iFrame "#". *)
+  (*     iDestruct "Hrel" as %Hrel. *)
+  (*     iPureIntro. apply region_state_nwl_monotone_a with W a0;auto. eapply region_addrs_lookup_le;eauto.  *)
+  (*   - iModIntro. iIntros (r W''). *)
+  (*     destruct l; simpl. *)
+  (*     + iIntros (Hrelated'). *)
+  (*       iAssert (future_world Global a W W'')%I as "Hrelated". *)
+  (*       { iPureIntro. apply related_sts_a_priv_trans_world with W' a0; auto. } *)
+  (*       iSpecialize ("Hw" $! r W'' with "Hrelated"). *)
+  (*       iApply "Hw". *)
+  (*     + iIntros (Hrelated'). *)
+  (*       iAssert (future_world Local a W W'')%I as "Hrelated". *)
+  (*       { iPureIntro. apply related_sts_a_priv_trans_world with W' a0; auto. } *)
+  (*       iSpecialize ("Hw" $! r W'' with "Hrelated"). *)
+  (*       iApply "Hw". *)
+  (*     + iIntros (Hrelated'). *)
+  (*       iAssert (future_world Directed a0 W W'')%I as "Hrelated". *)
+  (*       { iPureIntro. apply related_sts_a_trans_world with W';auto. } *)
+  (*       iSpecialize ("Hw" $! r W'' with "Hrelated"). *)
+  (*       iApply "Hw". *)
+  (*   - iApply (big_sepL_mono with "Hw"). *)
+  (*     iIntros (n y Hsome) "Hw". *)
+  (*     iDestruct "Hw" as "#[Hrw Hrel]". *)
+  (*     iSplit;eauto. iFrame "#". *)
+  (*     iDestruct "Hrel" as %Hrel. *)
+  (*     iPureIntro. apply region_state_nwl_monotone_a with W a0;auto. eapply region_addrs_lookup_le;eauto.  *)
+  (*   - destruct l; auto. *)
+  (*     iApply (big_sepL_mono with "Hw"). *)
+  (*     iIntros (n y Hsome) "Hw". *)
+  (*     iDestruct "Hw" as "#[Hrw Hrel]". *)
+  (*     iSplit;eauto. iFrame "#". *)
+  (*     iDestruct "Hrel" as %Hrel. *)
+  (*     iPureIntro. apply region_state_pwl_monotone_a with W a0;auto. eapply region_addrs_lookup_le;eauto.  *)
+  (*   - destruct l; simpl. *)
+  (*     + iApply (big_sepL_mono with "Hw"). *)
+  (*       iIntros (n y Hsome) "Hw". *)
+  (*       iDestruct "Hw" as "#[Hrw Hst]". *)
+  (*       iSplit;eauto. iFrame "#". *)
+  (*       iDestruct "Hst" as %Hst. *)
+  (*       iPureIntro. apply region_state_nwl_monotone_nm_nl with W;auto. *)
+  (*       apply related_sts_pub_plus_priv_world, related_sts_a_pub_plus_world with a;auto.  *)
+  (*     + iDestruct "Hw" as "[Hw1 Hw2]". *)
+  (*       iSplitL "Hw1". *)
+  (*       * iApply (big_sepL_mono with "Hw1"). *)
+  (*         iIntros (n y Hsome) "Hw". *)
+  (*         iDestruct "Hw" as "#[Hrw Hst ]". *)
+  (*         iSplit;eauto. iFrame "#". *)
+  (*         iDestruct "Hst" as %Hstd. *)
+  (*         iPureIntro. eapply (region_state_nwl_monotone_a W W' _ (addr_reg.min a a0) Local); auto. *)
+  (*         eapply region_addrs_lookup_le;eauto.  apply related_sts_a_weak_world with a;auto. solve_addr.  *)
+  (*       * iApply (big_sepL_mono with "Hw2"). *)
+  (*         iIntros (n y Hsome) "Hw". *)
+  (*         iDestruct "Hw" as "#[Hrw Hst ]". *)
+  (*         iSplit;eauto. iFrame "#". *)
+  (*         iDestruct "Hst" as %Hst. *)
+  (*         iPureIntro. *)
+  (*         eapply region_state_U_monotone; eauto. *)
+  (*         apply related_sts_pub_plus_priv_world. apply related_sts_a_pub_plus_world with a;auto. *)
+  (*     + iDestruct "Hw" as "[Hw1 Hw2]". *)
+  (*       iSplitL "Hw1". *)
+  (*       * iApply (big_sepL_mono with "Hw1"). *)
+  (*         iIntros (n y Hsome) "Hw". *)
+  (*         iDestruct "Hw" as "#[Hrw Hst ]". *)
+  (*         iSplit;eauto. iFrame "#". *)
+  (*         iDestruct "Hst" as %Hstd. *)
+  (*         iPureIntro. eapply (region_state_nwl_monotone_a W W' _ (addr_reg.min a a0) Directed); auto. *)
+  (*         eapply region_addrs_lookup_le;eauto.  apply related_sts_a_weak_world with a;auto. solve_addr. *)
+  (*       * iApply (big_sepL_mono with "Hw2"). *)
+  (*         iIntros (n y Hsome) "Hw". *)
+  (*         iDestruct "Hw" as "#[Hrw Hst ]". *)
+  (*         iSplit;eauto. iFrame "#". *)
+  (*         iDestruct "Hst" as %Hst. *)
+  (*         iPureIntro. *)
+  (*         eapply region_state_U_monotone_mono; eauto. *)
+  (*         apply related_sts_a_pub_plus_world with a;auto. *)
+  (*   - destruct l; auto. *)
+  (*     iDestruct "Hw" as "[Hbe Hexec]". *)
+  (*     iSplit. *)
+  (*     { iApply (big_sepL_mono with "Hbe"). *)
+  (*       iIntros (n y Hsome) "Hw". *)
+  (*       iDestruct "Hw" as "#[Hrw Hrel ]". *)
+  (*       iSplit;eauto. iFrame "#". *)
+  (*       iDestruct "Hrel" as %Hrel. *)
+  (*       iPureIntro. apply region_state_pwl_monotone_a with W (addr_reg.min a a0);auto. *)
+  (*       eapply region_addrs_lookup_le;eauto. apply related_sts_a_weak_world with a;auto. solve_addr. *)
+  (*     } *)
+  (*     { iApply (big_sepL_mono with "Hexec"). *)
+  (*       iIntros (n y Hsome) "Hw". *)
+  (*       iDestruct "Hw" as "#[Hrw Hrel ]". *)
+  (*       iSplit;eauto. iFrame "#". *)
+  (*       iDestruct "Hrel" as %Hrel. *)
+  (*       iPureIntro. apply region_state_U_pwl_monotone_mono_a with W (addr_reg.min a a0);auto. *)
+  (*       apply related_sts_a_weak_world with a;auto. solve_addr. } *)
+  (*   - destruct l; simpl. *)
+  (*     + iApply (big_sepL_mono with "Hw"). *)
+  (*       iIntros (n y Hsome) "Hw". *)
+  (*       iDestruct "Hw" as "#[Hrw Hst ]". *)
+  (*       iSplit;eauto. iFrame "#". *)
+  (*       iDestruct "Hst" as %Hst. *)
+  (*       iPureIntro. apply region_state_nwl_monotone_nm_nl with W;auto. *)
+  (*       apply related_sts_pub_plus_priv_world, related_sts_a_pub_plus_world with a;auto. *)
+  (*     + iDestruct "Hw" as "[Hw1 Hw2]". *)
+  (*       iSplitL "Hw1". *)
+  (*       * iApply (big_sepL_mono with "Hw1"). *)
+  (*         iIntros (n y Hsome) "Hw". *)
+  (*         iDestruct "Hw" as "#[Hrw Hst ]". *)
+  (*         iSplit;eauto. iFrame "#". *)
+  (*         iDestruct "Hst" as %Hstd. *)
+  (*         iPureIntro. eapply (region_state_nwl_monotone_a W W' _ (addr_reg.min a a0) Local); auto. *)
+  (*         eapply region_addrs_lookup_le;eauto. apply related_sts_a_weak_world with a;auto. solve_addr. *)
+  (*       * iApply (big_sepL_mono with "Hw2"). *)
+  (*         iIntros (n y Hsome) "Hw". *)
+  (*         iDestruct "Hw" as "#[Hrw Hst ]". *)
+  (*         iSplit;eauto. iFrame "#". *)
+  (*         iDestruct "Hst" as %Hst. *)
+  (*         iPureIntro. *)
+  (*         eapply region_state_U_monotone; eauto. *)
+  (*         apply related_sts_pub_plus_priv_world. *)
+  (*         apply related_sts_a_pub_plus_world with a;auto. *)
+  (*     + iDestruct "Hw" as "[Hw1 Hw2]". *)
+  (*       iSplitL "Hw1". *)
+  (*       * iApply (big_sepL_mono with "Hw1"). *)
+  (*         iIntros (n y Hsome) "Hw". *)
+  (*         iDestruct "Hw" as "#[Hrw Hst ]". *)
+  (*         iSplit;eauto. iFrame "#". *)
+  (*         iDestruct "Hst" as %Hstd. *)
+  (*         iPureIntro. eapply (region_state_nwl_monotone_a W W' _ (addr_reg.min a a0)  Directed); auto. *)
+  (*         eapply region_addrs_lookup_le;eauto. apply related_sts_a_weak_world with a;auto. solve_addr. *)
+  (*        * iApply (big_sepL_mono with "Hw2"). *)
+  (*         iIntros (n y Hsome) "Hw". *)
+  (*         iDestruct "Hw" as "#[Hrw Hst ]". *)
+  (*         iSplit;eauto. iFrame "#". *)
+  (*         iDestruct "Hst" as %Hst. *)
+  (*         iPureIntro. *)
+  (*         eapply region_state_U_monotone_mono; eauto. *)
+  (*         apply related_sts_a_pub_plus_world with a;auto. *)
+  (*   - destruct l; auto. *)
+  (*     iDestruct "Hw" as "[Hbe Hexec]". *)
+  (*     iSplit. *)
+  (*     { iApply (big_sepL_mono with "Hbe"). *)
+  (*       iIntros (n y Hsome) "Hw". *)
+  (*       iDestruct "Hw" as "#[Hrw Hrel ]". *)
+  (*       iSplit;eauto. iFrame "#". *)
+  (*       iDestruct "Hrel" as %Hrel. *)
+  (*       iPureIntro. apply region_state_pwl_monotone_a with W (addr_reg.min a a0);auto. *)
+  (*       eapply region_addrs_lookup_le;eauto. apply related_sts_a_weak_world with a;auto. solve_addr. *)
+  (*     } *)
+  (*     { iApply (big_sepL_mono with "Hexec"). *)
+  (*       iIntros (n y Hsome) "Hw". *)
+  (*       iDestruct "Hw" as "#[Hrw Hrel ]". *)
+  (*       iSplit;eauto. iFrame "#". *)
+  (*       iDestruct "Hrel" as %Hrel. *)
+  (*       iPureIntro. apply region_state_U_pwl_monotone_mono_a with W a;auto. } *)
+  (* Qed. *)
 
-  Definition isDirectedWord (w : Word) :=
-    match w with
-    | inl _ => false
-    | inr (_,l,_,_,_) => isDirected l
-    end.
+  (* Definition isDirectedWord (w : Word) := *)
+  (*   match w with *)
+  (*   | inl _ => false *)
+  (*   | inr (_,l,_,_,_) => isDirected l *)
+  (*   end. *)
 
-  Lemma interp_monotone_nm W W' w :
-    ⌜related_sts_priv_world W W'⌝ -∗ ⌜isDirectedWord w = false⌝ -∗
-    interp W w -∗ interp W' w.
-  Proof.
-    iIntros (Hrelated Hnl) "#Hw".
-    rewrite /interp /= fixpoint_interp1_eq /=.
-    destruct w; rewrite fixpoint_interp1_eq /=; auto.
-    destruct c,p,p,p,p; auto.
-    - iApply (big_sepL_mono with "Hw").
-      iIntros (n y Hsome) "Hw".
-      iDestruct "Hw" as (p Hpers) "#[Hrw Hrel ]".
-      iExists _. iSplit;eauto. iFrame "#".
-      iDestruct "Hrel" as %Hrel.
-      iPureIntro. destruct l; try discriminate.
-      apply region_state_nwl_monotone_nm_nl with W;auto.
-      apply region_state_nwl_monotone_nm with W;auto.
-    - iApply (big_sepL_mono with "Hw").
-      iIntros (n y Hsome) "Hw".
-      iDestruct "Hw" as "#[Hrw Hrel ]".
-      iSplit;eauto. iFrame "#".
-      iDestruct "Hrel" as %Hrel.
-      iPureIntro. destruct l; try discriminate.
-      apply region_state_nwl_monotone_nm_nl with W;auto.
-      apply region_state_nwl_monotone_nm with W;auto.
-    - destruct l; auto. discriminate.
-    - iApply (big_sepL_mono with "Hw").
-      iIntros (n y Hsome) "Hw".
-      iDestruct "Hw" as (p Hpers) "#[Hrw Hrel ]".
-      iExists _. iSplit;eauto. iFrame "#".
-      iDestruct "Hrel" as %Hrel.
-      iPureIntro. destruct l; try discriminate.
-      apply region_state_nwl_monotone_nm_nl with W;auto.
-      apply region_state_nwl_monotone_nm with W;auto.
-    - iModIntro. iIntros (r W'').
-      destruct l; simpl; try discriminate.
-      + iIntros (Hrelated').
-        iAssert (future_world Global a W W'')%I as "Hrelated".
-        { iPureIntro. apply related_sts_priv_trans_world with W'; auto. }
-        iSpecialize ("Hw" $! r W'' with "Hrelated").
-        iApply "Hw".
-      + iIntros (Hrelated').
-        iAssert (future_world Local a W W'')%I as "Hrelated".
-        { iPureIntro. apply related_sts_priv_trans_world with W'; auto. }
-        iSpecialize ("Hw" $! r W'' with "Hrelated").
-        iApply "Hw".
-    - iApply (big_sepL_mono with "Hw").
-      iIntros (n y Hsome) "Hw".
-      iDestruct "Hw" as "#[Hrw Hrel ]".
-      iSplit;eauto. iFrame "#".
-      iDestruct "Hrel" as %Hrel.
-      iPureIntro. destruct l; try discriminate.
-      apply region_state_nwl_monotone_nm_nl with W;auto.
-      apply region_state_nwl_monotone_nm with W;auto.
-    - destruct l; try discriminate. done. done.
-    - destruct l; simpl in Hnl; try discriminate.
-      + iApply (big_sepL_mono with "Hw").
-        iIntros (n y Hsome) "Hw".
-        iDestruct "Hw" as "#[Hrw Hst ]".
-        iSplit;eauto. iFrame "#".
-        iDestruct "Hst" as %Hst.
-        iPureIntro.
-        apply region_state_nwl_monotone_nm_nl with W;auto.
-      + iDestruct "Hw" as "[Hw1 Hw2]".
-        iSplit.
-        { iApply (big_sepL_mono with "Hw1").
-          iIntros (n y Hsome) "Hw".
-          iDestruct "Hw" as "#[Hrw Hst ]".
-          iSplit;eauto. iFrame "#".
-          iDestruct "Hst" as %Hst.
-          iPureIntro.
-          apply region_state_nwl_monotone_nm with W;auto. }
-        { iApply (big_sepL_mono with "Hw2").
-          iIntros (n y Hsome) "Hw".
-          iDestruct "Hw" as "#[Hrw Hst ]".
-          iSplit;eauto. iFrame "#".
-          iDestruct "Hst" as %Hst.
-          iPureIntro.
-          apply region_state_U_monotone with W;auto. }
-    - destruct l; auto. discriminate.
-    - destruct l; simpl in Hnl; try discriminate.
-      + iApply (big_sepL_mono with "Hw").
-        iIntros (n y Hsome) "Hw".
-        iDestruct "Hw" as "#[Hrw Hst ]".
-        iSplit;eauto. iFrame "#".
-        iDestruct "Hst" as %Hst.
-        iPureIntro.
-        apply region_state_nwl_monotone_nm_nl with W; auto.
-      + iDestruct "Hw" as "[Hw1 Hw2]".
-        iSplit.
-        { iApply (big_sepL_mono with "Hw1").
-          iIntros (n y Hsome) "Hw".
-          iDestruct "Hw" as "#[Hrw Hst ]".
-          iSplit;eauto. iFrame "#".
-          iDestruct "Hst" as %Hst.
-          iPureIntro.
-          apply region_state_nwl_monotone_nm with W;auto. }
-        { iApply (big_sepL_mono with "Hw2").
-          iIntros (n y Hsome) "Hw".
-          iDestruct "Hw" as "#[Hrw Hst ]".
-          iSplit;eauto. iFrame "#".
-          iDestruct "Hst" as %Hst.
-          iPureIntro.
-          apply region_state_U_monotone with W;auto. }
-    - destruct l; try discriminate. done. done.
-  Qed.
+  (* Lemma interp_monotone_nm W W' w : *)
+  (*   ⌜related_sts_priv_world W W'⌝ -∗ *)
+  (*   interp W w -∗ interp W' w. *)
+  (* Proof. *)
+  (*   iIntros (Hrelated) "#Hw". *)
+  (*   rewrite /interp /= fixpoint_interp1_eq /=. *)
+  (*   destruct w; rewrite fixpoint_interp1_eq /=; auto. *)
+  (*   destruct c,p,p,p,p; auto. *)
+  (*   - iApply (big_sepL_mono with "Hw"). *)
+  (*     iIntros (n y Hsome) "Hw". *)
+  (*     iDestruct "Hw" as (p Hpers) "#[Hrw Hrel ]". *)
+  (*     iExists _. iSplit;eauto. iFrame "#". *)
+  (*     iDestruct "Hrel" as %Hrel. *)
+  (*     iPureIntro. destruct l; try discriminate. *)
+  (*     apply region_state_nwl_monotone_nm_nl with W;auto. *)
+  (*     apply region_state_nwl_monotone_nm with W;auto. *)
+  (*   - iApply (big_sepL_mono with "Hw"). *)
+  (*     iIntros (n y Hsome) "Hw". *)
+  (*     iDestruct "Hw" as "#[Hrw Hrel ]". *)
+  (*     iSplit;eauto. iFrame "#". *)
+  (*     iDestruct "Hrel" as %Hrel. *)
+  (*     iPureIntro. destruct l; try discriminate. *)
+  (*     apply region_state_nwl_monotone_nm_nl with W;auto. *)
+  (*     apply region_state_nwl_monotone_nm with W;auto. *)
+  (*   - admit. *)
+  (*   (* - destruct l eqn:Hl; auto. *) *)
+  (*     (* discriminate. *) *)
+  (*   - iApply (big_sepL_mono with "Hw"). *)
+  (*     iIntros (n y Hsome) "Hw". *)
+  (*     iDestruct "Hw" as (p Hpers) "#[Hrw Hrel ]". *)
+  (*     iExists _. iSplit;eauto. iFrame "#". *)
+  (*     iDestruct "Hrel" as %Hrel. *)
+  (*     iPureIntro. *)
+  (*     destruct l; try discriminate. *)
+  (*     apply region_state_nwl_monotone_nm_nl with W;auto. *)
+  (*     apply region_state_nwl_monotone_nm with W;auto. *)
+  (*   - iModIntro. iIntros (r W''). *)
+  (*     destruct l; simpl; try discriminate. *)
+  (*     + iIntros (Hrelated'). *)
+  (*       iAssert (future_world Global W W'')%I as "Hrelated". *)
+  (*       { iPureIntro. apply related_sts_priv_trans_world with W'; auto. } *)
+  (*       iSpecialize ("Hw" $! r W'' with "Hrelated"). *)
+  (*       iApply "Hw". *)
+  (*     + iIntros (Hrelated'). *)
+  (*       iAssert (future_world Local W W'')%I as "Hrelated". *)
+  (*       { iPureIntro. apply related_sts_priv_trans_world with W'; auto. } *)
+  (*       iSpecialize ("Hw" $! r W'' with "Hrelated"). *)
+  (*       iApply "Hw". *)
+  (*   - iApply (big_sepL_mono with "Hw"). *)
+  (*     iIntros (n y Hsome) "Hw". *)
+  (*     iDestruct "Hw" as "#[Hrw Hrel ]". *)
+  (*     iSplit;eauto. iFrame "#". *)
+  (*     iDestruct "Hrel" as %Hrel. *)
+  (*     iPureIntro. destruct l; try discriminate. *)
+  (*     apply region_state_nwl_monotone_nm_nl with W;auto. *)
+  (*     apply region_state_nwl_monotone_nm with W;auto. *)
+  (*   (* - destruct l; try discriminate. done. done. *) *)
+  (*   - destruct l; try done. *)
+  (*     + iApply (big_sepL_mono with "Hw"). *)
+  (*       iIntros (n y Hsome) "Hw". *)
+  (*       iDestruct "Hw" as (p) "(%Hp & #Hrw & # Hst)". *)
+  (*       iExists p. *)
+  (*       iSplit;eauto. iFrame "#". *)
+  (*       iDestruct "Hst" as %Hst. *)
+  (*       iPureIntro. *)
+  (*       admit. *)
+  (*       (* apply region_state_nwl_monotone_nm_nl with W;auto. *) *)
+  (*     (* + iDestruct "Hw" as "[Hw1 Hw2]". *) *)
+  (*     (*   iSplit. *) *)
+  (*     (*   { iApply (big_sepL_mono with "Hw1"). *) *)
+  (*     (*     iIntros (n y Hsome) "Hw". *) *)
+  (*     (*     iDestruct "Hw" as "#[Hrw Hst ]". *) *)
+  (*     (*     iSplit;eauto. iFrame "#". *) *)
+  (*     (*     iDestruct "Hst" as %Hst. *) *)
+  (*     (*     iPureIntro. *) *)
+  (*     (*     apply region_state_nwl_monotone_nm with W;auto. } *) *)
+  (*     (*   { iApply (big_sepL_mono with "Hw2"). *) *)
+  (*     (*     iIntros (n y Hsome) "Hw". *) *)
+  (*     (*     iDestruct "Hw" as "#[Hrw Hst ]". *) *)
+  (*     (*     iSplit;eauto. iFrame "#". *) *)
+  (*     (*     iDestruct "Hst" as %Hst. *) *)
+  (*     (*     iPureIntro. *) *)
+  (*         (* apply region_state_U_monotone with W;auto. } *) *)
+  (*   - destruct l; auto. discriminate. *)
+  (*   - destruct l; simpl in Hnl; try discriminate. *)
+  (*     + iApply (big_sepL_mono with "Hw"). *)
+  (*       iIntros (n y Hsome) "Hw". *)
+  (*       iDestruct "Hw" as "#[Hrw Hst ]". *)
+  (*       iSplit;eauto. iFrame "#". *)
+  (*       iDestruct "Hst" as %Hst. *)
+  (*       iPureIntro. *)
+  (*       apply region_state_nwl_monotone_nm_nl with W; auto. *)
+  (*     + iDestruct "Hw" as "[Hw1 Hw2]". *)
+  (*       iSplit. *)
+  (*       { iApply (big_sepL_mono with "Hw1"). *)
+  (*         iIntros (n y Hsome) "Hw". *)
+  (*         iDestruct "Hw" as "#[Hrw Hst ]". *)
+  (*         iSplit;eauto. iFrame "#". *)
+  (*         iDestruct "Hst" as %Hst. *)
+  (*         iPureIntro. *)
+  (*         apply region_state_nwl_monotone_nm with W;auto. } *)
+  (*       { iApply (big_sepL_mono with "Hw2"). *)
+  (*         iIntros (n y Hsome) "Hw". *)
+  (*         iDestruct "Hw" as "#[Hrw Hst ]". *)
+  (*         iSplit;eauto. iFrame "#". *)
+  (*         iDestruct "Hst" as %Hst. *)
+  (*         iPureIntro. *)
+  (*         apply region_state_U_monotone with W;auto. } *)
+  (*   - destruct l; try discriminate. done. done. *)
+  (* Qed. *)
 
-(*  Lemma interp_monotone_nm_nl W W' w :
+ Lemma interp_monotone_nm_nl W W' w :
     ⌜related_sts_priv_world W W'⌝ -∗ ⌜isLocalWord w = false⌝ -∗
     interp W w -∗ interp W' w.
   Proof.
@@ -789,8 +652,9 @@ Section monotone.
       apply region_state_nwl_monotone_nm_nl with W;auto.
     - iApply (big_sepL_mono with "Hw").
       iIntros (n y Hsome) "Hw".
-      iDestruct "Hw" as (p Hfl) "#[Hrw Hrel ]".
-      iExists _. iSplit;eauto. iFrame "#".
+      iDestruct "Hw" as "#[Hrw Hrel ]".
+      (* iDestruct "Hw" as (p Hfl) "#[Hrw Hrel ]". *)
+      iSplit;eauto. iFrame "#".
       iDestruct "Hrel" as %Hrel.
       iPureIntro. destruct l; try discriminate.
       apply region_state_nwl_monotone_nm_nl with W;auto.
@@ -805,49 +669,30 @@ Section monotone.
     - iModIntro. iIntros (r W'').
       destruct l; simpl; try discriminate.
       iIntros (Hrelated').
-      iAssert (future_world Global a0 W W'')%I as "Hrelated".
+      iAssert (future_world Global W W'')%I as "Hrelated".
       { iPureIntro. apply related_sts_priv_trans_world with W'; auto. }
       iSpecialize ("Hw" $! r W'' with "Hrelated").
       iApply "Hw".
     - iApply (big_sepL_mono with "Hw").
       iIntros (n y Hsome) "Hw".
-      iDestruct "Hw" as (p Hfl) "#[Hrw Hrel ]".
-      iExists _. iSplit;eauto. iFrame "#".
+      iDestruct "Hw" as "#[Hrw Hrel ]".
+      iSplit;eauto. iFrame "#".
       iDestruct "Hrel" as %Hrel.
       iPureIntro. destruct l; try discriminate.
       apply region_state_nwl_monotone_nm_nl with W;auto.
     - destruct l; try discriminate. done.
-    - destruct l; simpl in Hnl; try discriminate.
-      iApply (big_sepL_mono with "Hw").
-      iIntros (n y Hsome) "Hw".
-      iDestruct "Hw" as (p Hfl) "#[Hrw Hst ]".
-      iExists _. iSplit;eauto. iFrame "#".
-      iDestruct "Hst" as %Hst.
-      iPureIntro.
-      apply region_state_nwl_monotone_nm_nl with W; auto.
-    - destruct l; auto. discriminate.
-    - destruct l; simpl in Hnl; try discriminate.
-      iApply (big_sepL_mono with "Hw").
-      iIntros (n y Hsome) "Hw".
-      iDestruct "Hw" as (p Hfl) "#[Hrw Hst ]".
-      iExists _. iSplit;eauto. iFrame "#".
-      iDestruct "Hst" as %Hst.
-      iPureIntro.
-      apply region_state_nwl_monotone_nm_nl with W; auto.
-    - destruct l; try discriminate. done.
-  Qed.*)
+  Qed.
 
   (*Lemma that allows switching between the two different formulations of monotonicity, to alleviate the effects of inconsistencies*)
   Lemma switch_monotonicity_formulation ρ l w φ:
-      ρ ≠ Revoked → (∀ m, ρ ≠ Monostatic m) -> (∀ w, ρ ≠ Uninitialized w) ->
+      ρ ≠ Revoked → (∀ m, ρ ≠ Monostatic m) ->
       monotonicity_guarantees_region ρ l w φ ≡ monotonicity_guarantees_decide (Σ := Σ) ρ l w φ.
   Proof.
-    intros Hrev Hmono Huninit.
+    intros Hrev Hmono.
     unfold monotonicity_guarantees_region, monotonicity_guarantees_decide.
     iSplit; iIntros "HH".
     - destruct ρ;simpl;auto;try done.
       * specialize (Hmono g). done.
-      * specialize (Huninit w0). done.
     - intros. destruct ρ;simpl;auto.
   Qed.
 
@@ -871,9 +716,9 @@ Section monotone.
   Lemma adv_stack_monotone W W' b e :
     related_sts_pub_world W W' ->
     ([∗ list] a ∈ region_addrs b e, read_write_cond a interp
-                                     ∧ ⌜region_state_pwl_mono W a⌝)
+                                     ∧ ⌜region_state_pwl W a⌝)
     -∗ ([∗ list] a ∈ region_addrs b e, read_write_cond a interp
-                                       ∧ ⌜region_state_pwl_mono W' a⌝).
+                                       ∧ ⌜region_state_pwl W' a⌝).
   Proof.
     iIntros (Hrelated) "Hstack_adv".
     iApply (big_sepL_mono with "Hstack_adv").
@@ -904,72 +749,70 @@ Proof.
   - iModIntro; simpl;auto.
     iIntros (W0 W1) "% HIW0".
     destruct g.
-    * iApply (interp_monotone_nm with "[] [] HIW0");auto.
+    * iApply (interp_monotone_nm_nl with "[] [] HIW0");auto.
       iPureIntro.
       apply related_sts_a_pub_plus_world in H0.
       apply related_sts_pub_plus_priv_world;auto.
-    * iApply (interp_monotone_nm with "[] [] HIW0");auto.
-      iPureIntro. apply related_sts_pub_plus_priv_world. apply related_sts_a_pub_plus_world with a0;auto.
-    * destruct (decide (p = O)). 
-      { subst. rewrite !fixpoint_interp1_eq. done. }
-      iApply (interp_monotone_a with "[] HIW0");auto.
-      apply andb_prop in Hconds as [Hp0 Hleb].
-      simpl. destruct (isU p) eqn:Hu.
-      ** assert (a <= a0)%a as Hle.
-         { destruct p; inversion Hu;simpl in Hleb;apply Z.leb_le in Hleb;solve_addr. }
-         iPureIntro. apply related_sts_a_weak_world with a0;auto. 
-      ** assert (e <= a0)%a as Hle.
-         { destruct p; inversion Hu;simpl in Hleb;apply Z.leb_le in Hleb; try solve_addr. }
-         iPureIntro. apply related_sts_a_weak_world with a0;auto.
+    * admit.
+    (* * iApply (interp_monotone_nm_nl with "[] [] HIW0");auto. *)
+    (*   iPureIntro. apply related_sts_pub_plus_priv_world. apply related_sts_a_pub_plus_world with a0;auto. *)
+    (* * destruct (decide (p = O)). *)
+    (*   { subst. rewrite !fixpoint_interp1_eq. done. } *)
+    (*   iApply (interp_monotone_a with "[] HIW0");auto. *)
+    (*   apply andb_prop in Hconds as [Hp0 Hleb]. *)
+    (*   simpl. destruct (isU p) eqn:Hu. *)
+    (*   ** assert (a <= a0)%a as Hle. *)
+    (*      { destruct p; inversion Hu;simpl in Hleb;apply Z.leb_le in Hleb;solve_addr. } *)
+    (*      iPureIntro. apply related_sts_a_weak_world with a0;auto. *)
+    (*   ** assert (e <= a0)%a as Hle. *)
+    (*      { destruct p; inversion Hu;simpl in Hleb;apply Z.leb_le in Hleb; try solve_addr. } *)
+    (*      iPureIntro. apply related_sts_a_weak_world with a0;auto. *)
   - iModIntro. simpl. iIntros (W0 W1) "% HIW0".
     destruct g.
-    + by iApply interp_monotone_nm.
+    + by iApply interp_monotone_nm_nl.
     + (*Trick here: value relation leads to a contradiction if p0 is WL, since then its region cannot be permanent*)
       iDestruct ( writeLocalAllowed_valid_cap_implies with "Hvdst" ) as %Ha; eauto.
       rewrite Hstd in Ha. inversion Ha.
-    + apply andb_prop in Hconds as [Hp0 Hleb].
-      iDestruct ( writeLocalAllowed_valid_cap_implies with "Hvdst" ) as %Ha; eauto.
-      rewrite Hstd in Ha. inversion Ha.
-Qed.
+Admitted.
 
-Lemma interp_monotone_generalUW (W : WORLD)  (ρ : region_type) (p p0 : Perm) (l g : Locality)(b e a a2 a1 a0 : Addr):
-  std W !! a0 = Some ρ →
-  withinBounds (p0, l, a2, a1, a0) = true →
-  canStoreU p0 a0 (inr (p,g,b,e,a)) = true →
-  ((fixpoint interp1) W) (inr (p0, l, a2, a1, a0)) -∗
-  monotonicity_guarantees_region ρ a0 (inr (p, g, b, e, a))  (λne Wv : WORLD * (leibnizO Word), (interp Wv.1) Wv.2).
-Proof.
-  unfold monotonicity_guarantees_region.
-  iIntros (Hstd Hwb Hconds) "#Hvdst".
-  destruct ρ;auto.
-  - iModIntro; simpl;auto.
-    iIntros (W0 W1) "% HIW0".
-    destruct g.
-    * iApply (interp_monotone_nm with "[] [] HIW0");auto.
-      iPureIntro. apply related_sts_a_pub_plus_world in H0. apply related_sts_pub_plus_priv_world;auto.
-    * iApply (interp_monotone_nm with "[] [] HIW0");auto.
-      iPureIntro. apply related_sts_pub_plus_priv_world. apply related_sts_a_pub_plus_world with a0;auto.
-    * destruct (decide (p = O)). 
-      { subst. rewrite !fixpoint_interp1_eq. done. }
-      iApply (interp_monotone_a with "[] HIW0");auto.
-      apply andb_prop in Hconds as [Hp0 Hleb].
-      simpl. destruct (isU p) eqn:Hu.
-      ** assert (a <= a0)%a as Hle.
-         { destruct p; inversion Hu;simpl in Hleb;apply Z.leb_le in Hleb;solve_addr. }
-         iPureIntro. apply related_sts_a_weak_world with a0;auto. 
-      ** assert (e <= a0)%a as Hle.
-         { destruct p; inversion Hu;simpl in Hleb;apply Z.leb_le in Hleb; try solve_addr. }
-         iPureIntro. apply related_sts_a_weak_world with a0;auto.
-  - iModIntro. simpl. iIntros (W0 W1) "% HIW0".
-    destruct g.
-    + by iApply interp_monotone_nm.
-    + (*Trick here: value relation leads to a contradiction if p0 is WL, since then its region cannot be permanent*)
-      iDestruct ( writeLocalAllowedU_valid_cap_implies with "Hvdst" ) as %Ha; eauto.
-      destruct Ha as [Ha | [? Ha] ]; rewrite Hstd in Ha; inversion Ha.
-    + apply andb_prop in Hconds as [Hp0 Hleb].
-      iDestruct ( writeLocalAllowedU_valid_cap_implies with "Hvdst" ) as %Ha; eauto.
-      destruct Ha as [Ha | [? Ha] ]; rewrite Hstd in Ha; inversion Ha.
-Qed.
+(* Lemma interp_monotone_generalUW (W : WORLD)  (ρ : region_type) (p p0 : Perm) (l g : Locality)(b e a a2 a1 a0 : Addr): *)
+(*   std W !! a0 = Some ρ → *)
+(*   withinBounds (p0, l, a2, a1, a0) = true → *)
+(*   canStoreU p0 a0 (inr (p,g,b,e,a)) = true → *)
+(*   ((fixpoint interp1) W) (inr (p0, l, a2, a1, a0)) -∗ *)
+(*   monotonicity_guarantees_region ρ a0 (inr (p, g, b, e, a))  (λne Wv : WORLD * (leibnizO Word), (interp Wv.1) Wv.2). *)
+(* Proof. *)
+(*   unfold monotonicity_guarantees_region. *)
+(*   iIntros (Hstd Hwb Hconds) "#Hvdst". *)
+(*   destruct ρ;auto. *)
+(*   - iModIntro; simpl;auto. *)
+(*     iIntros (W0 W1) "% HIW0". *)
+(*     destruct g. *)
+(*     * iApply (interp_monotone_nm with "[] [] HIW0");auto. *)
+(*       iPureIntro. apply related_sts_a_pub_plus_world in H0. apply related_sts_pub_plus_priv_world;auto. *)
+(*     * iApply (interp_monotone_nm with "[] [] HIW0");auto. *)
+(*       iPureIntro. apply related_sts_pub_plus_priv_world. apply related_sts_a_pub_plus_world with a0;auto. *)
+(*     * destruct (decide (p = O)).  *)
+(*       { subst. rewrite !fixpoint_interp1_eq. done. } *)
+(*       iApply (interp_monotone_a with "[] HIW0");auto. *)
+(*       apply andb_prop in Hconds as [Hp0 Hleb]. *)
+(*       simpl. destruct (isU p) eqn:Hu. *)
+(*       ** assert (a <= a0)%a as Hle. *)
+(*          { destruct p; inversion Hu;simpl in Hleb;apply Z.leb_le in Hleb;solve_addr. } *)
+(*          iPureIntro. apply related_sts_a_weak_world with a0;auto.  *)
+(*       ** assert (e <= a0)%a as Hle. *)
+(*          { destruct p; inversion Hu;simpl in Hleb;apply Z.leb_le in Hleb; try solve_addr. } *)
+(*          iPureIntro. apply related_sts_a_weak_world with a0;auto. *)
+(*   - iModIntro. simpl. iIntros (W0 W1) "% HIW0". *)
+(*     destruct g. *)
+(*     + by iApply interp_monotone_nm. *)
+(*     + (*Trick here: value relation leads to a contradiction if p0 is WL, since then its region cannot be permanent*) *)
+(*       iDestruct ( writeLocalAllowedU_valid_cap_implies with "Hvdst" ) as %Ha; eauto. *)
+(*       destruct Ha as [Ha | [? Ha] ]; rewrite Hstd in Ha; inversion Ha. *)
+(*     + apply andb_prop in Hconds as [Hp0 Hleb]. *)
+(*       iDestruct ( writeLocalAllowedU_valid_cap_implies with "Hvdst" ) as %Ha; eauto. *)
+(*       destruct Ha as [Ha | [? Ha] ]; rewrite Hstd in Ha; inversion Ha. *)
+(* Qed. *)
 
 (* Analogous, but now we have the general monotonicity statement in case an integer z is written *)
 Lemma interp_monotone_generalZ (W : WORLD)  (ρ : region_type) (p0 : Perm) (l : Locality)(a2 a1 a0 : Addr) z:
@@ -988,7 +831,6 @@ Proof.
     all: iIntros (W0 W1) "% HIW0".
     all: rewrite !fixpoint_interp1_eq;done.
 Qed.
-
 
 
 End monotone.
