theories/rules/rules_Store.v
@@ -238,28 +238,10 @@ Section cap_lang_rules.
      }
 
 
-     (* destruct (decide (isLocalWord storev = true ∧ pwl p = false)). *)
-     (* {  (* Failure: trying to write a local value to a non-WL cap *) *)
-     (*        destruct a0 as [HLW Hpwl]. *)
-     (*   assert (c = Failed ∧ σ2 = (r, m)) as (-> & ->). *)
-     (*  { destruct storev. *)
-     (*   - cbv in HLW; by exfalso. *)
-     (*   - destruct (word_of_argument_inr _ _ _ HSVr) as (r0 & -> & Hr0s). *)
-     (*     destruct (isLocalWord_cap_isLocal _ HLW) as (p' & g' & b' & e' & a' & -> & HIL). *)
-     (*     option_locate_mr m r. rewrite /canStore  Hrr0 /= Hpwl in Hstep. *)
-     (*     destruct g'; simpl in HIL; try congruence; inversion Hstep; auto. } *)
-     (*  iFailWP "Hφ" Store_fail_invalid_locality. *)
-     (* } *)
-
      assert (isLocalWord storev = false ∨ machine_base.pwl p = true) as HLocal.
      { rewrite /canStore in HcanStore. destruct storev; simpl; auto.
-       destruct_cap c0. destruct g0; auto.
-       eapply andb_true_iff in HcanStore. destruct HcanStore; auto. }
-     (* apply (not_and_r) in n0. *)
-     (* destruct n0 as [Hlw | Hpwl]. *)
-     (* destruct (isLocalWord storev); first by exfalso. by left. *)
-     (* destruct (pwl p); last by exfalso. by right. *)
-     (* } clear n0. *)
+       destruct_cap c0. destruct g0; auto. }
+       (* eapply andb_true_iff in HcanStore. destruct HcanStore; auto. } *)
 
      (* Prove that a is in the memory map now, otherwise we cannot continue *)
      pose proof (allow_store_implies_storev r1 r2 mem regs p g b e a storev) as (oldv & Hmema); auto.
@@ -308,7 +290,7 @@ Section cap_lang_rules.
       iPureIntro. eapply Store_spec_success; eauto.
         * split; auto. exact Hr'1. all: auto.
         * unfold incrementPC. rewrite HPC'' Ha_pc'.
-          destruct X as [? [? [? [? ?]]]]; destruct p1; auto; congruence.
+          destruct p1; auto; congruence.
       Unshelve. all: auto.
    Qed.
 
@@ -349,7 +331,7 @@ Section cap_lang_rules.
        apply isCorrectPC_ra_wb in Hvpc. apply andb_prop_elim in Hvpc as [_ Hwb].
        destruct o; last apply Is_true_false_2 in H2. all:try congruence.
        destruct e; try congruence.
-       inv Hvpc. destruct H2 as [? | [? | [? | [? | ?]]]]; destruct H9 as [? | [? | ?]]; congruence.
+       inv Hvpc.
      }
    Qed.
 
@@ -394,279 +376,9 @@ Section cap_lang_rules.
        destruct Hfail; try incrementPC_inv; simplify_map_eq; eauto.
        destruct o. all: try congruence.
        destruct e0; try congruence.
-       inv Hvpc. destruct H3 as [? | [? | [? | [? | ?]]]]; destruct H10 as [? | [? | ?]]; congruence.
+       inv Hvpc. destruct H10 as [? | [? | ?]]; congruence.
      }
     Qed.
-
-   (* Lemma wp_store_success_reg' E pc_p pc_g pc_b pc_e pc_a pc_a' w dst w' *)
-   (*       p g b e a pc_p' p' : *)
-   (*    decodeInstrW w = Store dst (inr PC) → *)
-   (*    PermFlows pc_p pc_p' → *)
-   (*   isCorrectPC (inr ((pc_p,pc_g),pc_b,pc_e,pc_a)) → *)
-   (*   (pc_a + 1)%a = Some pc_a' → *)
-   (*   writeAllowed p = true ∧ withinBounds ((p, g), b, e, a) = true → *)
-   (*   (isLocal pc_g = false ∨ (p = RWLX ∨ p = RWL)) → *)
-
-   (*   {{{ ▷ PC ↦ᵣ inr ((pc_p,pc_g),pc_b,pc_e,pc_a) *)
-   (*         ∗ ▷ pc_a ↦ₐ[pc_p'] w *)
-   (*         ∗ ▷ dst ↦ᵣ inr ((p,g),b,e,a) *)
-   (*         ∗ if (a =? pc_a)%a *)
-   (*           then ⌜PermFlows p pc_p'⌝ *)
-   (*           else ⌜PermFlows p p'⌝ ∗ ▷ a ↦ₐ[p'] w' }}} *)
-   (*     Instr Executable @ E *)
-   (*     {{{ RET NextIV; *)
-   (*         PC ↦ᵣ inr ((pc_p,pc_g),pc_b,pc_e,pc_a') *)
-   (*            ∗ pc_a ↦ₐ[pc_p'] (if (a =? pc_a)%a *)
-   (*                             then (inr ((pc_p,pc_g),pc_b,pc_e,pc_a)) *)
-   (*                             else w) *)
-   (*            ∗ dst ↦ᵣ inr ((p,g),b,e,a) *)
-   (*            ∗ if (a =? pc_a)%a *)
-   (*              then emp *)
-   (*              else a ↦ₐ[p'] (inr ((pc_p,pc_g),pc_b,pc_e,pc_a)) }}}. *)
-   (* Proof. *)
-   (*   iIntros (Hinstr Hfl Hvpc Hpca' [Hwa Hwb] Hloc φ) *)
-   (*          "(>HPC & >Hi & >Hdst & Ha) Hφ". *)
-   (*   iDestruct (map_of_regs_2 with "HPC Hdst") as "[Hmap %]". *)
-   (*   iDestruct (extract_sep_if_split with "Ha") as "[Hflt Hr1a]". *)
-   (*   iAssert (⌜if (a =? pc_a)%a then PermFlows p pc_p' else PermFlows p p'⌝)%I with "[Hflt]" as %Hfl'. *)
-   (*   { iRevert "Hflt". destruct (a =? pc_a)%a; auto. } *)
-   (*   iDestruct (memMap_resource_2gen_clater with "Hi Hr1a") as (mem) "[>Hmem %]". *)
-
-   (*  iApply (wp_store with "[$Hmap $Hmem]"); eauto; simplify_map_eq; eauto. *)
-   (*  { by rewrite !dom_insert; set_solver+. } *)
-   (*  { destruct (a =? pc_a)%a; by simplify_map_eq. } *)
-   (*  { eapply mem_implies_allow_store_map; eauto. all: by simplify_map_eq. } *)
-
-   (*  iNext. iIntros (regs' mem' retv) "(#Hspec & Hmem & Hmap)". *)
-   (*  iDestruct "Hspec" as %Hspec. *)
-
-   (*  destruct Hspec as [ | * Hfail ]. *)
-   (*   { (* Success *) *)
-   (*     iApply "Hφ". *)
-   (*     destruct H5 as [Hrr2 _]. simplify_map_eq. *)
-   (*     destruct (a0 =? pc_a)%a eqn:Heq; subst mem. *)
-   (*     -  apply Z.eqb_eq, z_of_eq in Heq. subst a0. *)
-   (*        rewrite insert_insert. *)
-   (*        rewrite memMap_resource_1. *)
-   (*        incrementPC_inv. *)
-   (*        simplify_map_eq. rewrite insert_insert. *)
-   (*        iDestruct (regs_of_map_2 with "[$Hmap]") as "[HPC Hsrc]"; eauto. iFrame. *)
-
-   (*     - apply Z.eqb_neq in Heq. *)
-   (*       rewrite insert_commute; last congruence. rewrite insert_insert. *)
-   (*       iDestruct (memMap_resource_2ne with "Hmem") as "[Ha0 Hpc_a]"; first congruence. *)
-   (*       incrementPC_inv. *)
-   (*       rewrite lookup_insert_ne in H6; last congruence. simplify_map_eq. rewrite insert_insert. *)
-   (*       iDestruct (regs_of_map_2 with "[$Hmap]") as "[HPC Hsrc]"; eauto. iFrame. *)
-   (*   } *)
-   (*   { (* Failure (contradiction) *) *)
-   (*     destruct Hfail; try incrementPC_inv; simplify_map_eq; eauto. *)
-   (*     destruct o. all: try congruence. *)
-   (*     destruct Hloc; first congruence. naive_solver. *)
-   (*   } *)
-   (*   Qed. *)
-
-   (* Lemma wp_store_success_reg_same' E pc_p pc_g pc_b pc_e pc_a pc_a' w dst *)
-   (*       p g b e pc_p' : *)
-   (*   decodeInstrW w = Store dst (inr dst) → *)
-   (*   PermFlows pc_p pc_p' → *)
-   (*   PermFlows p pc_p' → *)
-   (*   isCorrectPC (inr ((pc_p,pc_g),pc_b,pc_e,pc_a)) → *)
-   (*   (pc_a + 1)%a = Some pc_a' → *)
-   (*   writeAllowed p = true ∧ withinBounds ((p, g), b, e, pc_a) = true → *)
-   (*   (isLocal g = false ∨ (p = RWLX ∨ p = RWL)) → *)
-
-   (*   {{{ ▷ PC ↦ᵣ inr ((pc_p,pc_g),pc_b,pc_e,pc_a) *)
-   (*         ∗ ▷ pc_a ↦ₐ[pc_p'] w *)
-   (*         ∗ ▷ dst ↦ᵣ inr ((p,g),b,e,pc_a) }}} *)
-   (*     Instr Executable @ E *)
-   (*     {{{ RET NextIV; *)
-   (*         PC ↦ᵣ inr ((pc_p,pc_g),pc_b,pc_e,pc_a') *)
-   (*            ∗ pc_a ↦ₐ[pc_p'] inr (p, g, b, e, pc_a) *)
-   (*            ∗ dst ↦ᵣ inr ((p,g),b,e,pc_a) }}}. *)
-   (* Proof. *)
-   (*   iIntros (Hinstr Hfl Hfl' Hvpc Hpca' [Hwa Hwb] Hloc φ) *)
-   (*          "(>HPC & >Hi & >Hdst) Hφ". *)
-   (*   iDestruct (map_of_regs_2 with "HPC Hdst") as "[Hmap %]". *)
-   (*   iDestruct (memMap_resource_1 with "Hi") as "Hmem". *)
-
-   (*  iApply (wp_store _ pc_p with "[$Hmap $Hmem]"); eauto; simplify_map_eq; eauto. *)
-   (*  { by rewrite !dom_insert; set_solver+. } *)
-   (*  { eapply mem_eq_implies_allow_store_map; eauto. *)
-   (*    all: by simplify_map_eq. } *)
-   (*  iNext. iIntros (regs' mem' retv) "(#Hspec & Hmem & Hmap)". *)
-   (*  iDestruct "Hspec" as %Hspec. *)
-
-   (*  destruct Hspec as [ | * Hfail ]. *)
-   (*   { (* Success *) *)
-   (*     iApply "Hφ". *)
-   (*     destruct H4 as [Hrr2 _]. simplify_map_eq. *)
-   (*     rewrite memMap_resource_1. *)
-   (*     incrementPC_inv. *)
-   (*     simplify_map_eq. *)
-   (*     do 2 rewrite insert_insert. *)
-   (*     iDestruct (regs_of_map_2 with "[$Hmap]") as "[HPC Hsrc]"; eauto. iFrame. } *)
-   (*   { (* Failure (contradiction) *) *)
-   (*     destruct Hfail; try incrementPC_inv; simplify_map_eq; eauto. *)
-   (*     destruct o. all: try congruence. *)
-   (*     destruct Hloc; first congruence. naive_solver. *)
-   (*   } *)
-   (* Qed. *)
-
-   (* Lemma wp_store_success_reg_same_a E pc_p pc_g pc_b pc_e pc_a pc_a' w dst src *)
-   (*       p g b e pc_p' w'' : *)
-   (*    decodeInstrW w = Store dst (inr src) → *)
-   (*    PermFlows pc_p pc_p' → *)
-   (*    PermFlows p pc_p' → *)
-   (*   isCorrectPC (inr ((pc_p,pc_g),pc_b,pc_e,pc_a)) → *)
-   (*   (pc_a + 1)%a = Some pc_a' → *)
-   (*   writeAllowed p = true ∧ withinBounds ((p, g), b, e, pc_a) = true → *)
-   (*   (isLocalWord w'' = false ∨ (p = RWLX ∨ p = RWL)) → *)
-
-   (*   {{{ ▷ PC ↦ᵣ inr ((pc_p,pc_g),pc_b,pc_e,pc_a) *)
-   (*         ∗ ▷ pc_a ↦ₐ[pc_p'] w *)
-   (*         ∗ ▷ src ↦ᵣ w'' *)
-   (*         ∗ ▷ dst ↦ᵣ inr ((p,g),b,e,pc_a) }}} *)
-   (*     Instr Executable @ E *)
-   (*     {{{ RET NextIV; *)
-   (*         PC ↦ᵣ inr ((pc_p,pc_g),pc_b,pc_e,pc_a') *)
-   (*            ∗ pc_a ↦ₐ[pc_p'] w'' *)
-   (*            ∗ src ↦ᵣ w'' *)
-   (*            ∗ dst ↦ᵣ inr ((p,g),b,e,pc_a)}}}. *)
-   (* Proof. *)
-   (*   iIntros (Hinstr Hfl Hfl' Hvpc Hpca' [Hwa Hwb] Hloc φ) *)
-   (*           "(>HPC & >Hi & >Hsrc & >Hdst) Hφ". *)
-   (*   iDestruct (map_of_regs_3 with "HPC Hsrc Hdst") as "[Hmap (%&%&%)]". *)
-   (*   iDestruct (memMap_resource_1 with "Hi") as "Hmem". *)
-
-   (*  iApply (wp_store _ pc_p with "[$Hmap $Hmem]"); eauto; simplify_map_eq; eauto. *)
-   (*  { by rewrite !dom_insert; set_solver+. } *)
-   (*  { eapply mem_eq_implies_allow_store_map; eauto. *)
-   (*    all: by simplify_map_eq. } *)
-   (*  iNext. iIntros (regs' mem' retv) "(#Hspec & Hmem & Hmap)". *)
-   (*  iDestruct "Hspec" as %Hspec. *)
-
-   (*  destruct Hspec as [ | * Hfail ]. *)
-   (*   { (* Success *) *)
-   (*     iApply "Hφ". *)
-   (*     destruct H6 as [Hrr2 _]. simplify_map_eq. *)
-   (*     rewrite memMap_resource_1. *)
-   (*     incrementPC_inv. *)
-   (*     simplify_map_eq. *)
-   (*     do 2 rewrite insert_insert. *)
-   (*     iDestruct (regs_of_map_3 with "[$Hmap]") as "[HPC [Hsrc Hdst] ]"; eauto. iFrame. } *)
-   (*   { (* Failure (contradiction) *) *)
-   (*     destruct Hfail; try incrementPC_inv; simplify_map_eq; eauto. *)
-   (*     destruct o. all: try congruence. *)
-   (*     destruct Hloc; first congruence. naive_solver. *)
-   (*   } *)
-   (* Qed. *)
-
-  (* Lemma wp_store_success_local_reg E pc_p pc_g pc_b pc_e pc_a pc_a' w dst src w' *)
-  (*        p g b e a p' g' b' e' a' pc_p' p'' : *)
-  (*   decodeInstrW w = Store dst (inr src) → *)
-  (*   PermFlows pc_p pc_p' → *)
-  (*   PermFlows p p'' → *)
-  (*    isCorrectPC (inr ((pc_p,pc_g),pc_b,pc_e,pc_a)) → *)
-  (*    (pc_a + 1)%a = Some pc_a' → *)
-  (*    writeAllowed p = true ∧ withinBounds ((p, g), b, e, a) = true → *)
-  (*    isLocal g' = true ∧ (p = RWLX ∨ p = RWL) → *)
-
-  (*    {{{ ▷ PC ↦ᵣ inr ((pc_p,pc_g),pc_b,pc_e,pc_a) *)
-  (*          ∗ ▷ pc_a ↦ₐ[pc_p'] w *)
-  (*          ∗ ▷ src ↦ᵣ inr ((p',g'),b',e',a') *)
-  (*          ∗ ▷ dst ↦ᵣ inr ((p,g),b,e,a) *)
-  (*          ∗ ▷ a ↦ₐ[p''] w' }}} *)
-  (*      Instr Executable @ E *)
-  (*      {{{ RET NextIV; *)
-  (*          PC ↦ᵣ inr ((pc_p,pc_g),pc_b,pc_e,pc_a') *)
-  (*             ∗ pc_a ↦ₐ[pc_p'] w *)
-  (*             ∗ src ↦ᵣ inr ((p',g'),b',e',a') *)
-  (*             ∗ dst ↦ᵣ inr ((p,g),b,e,a) *)
-  (*             ∗ a ↦ₐ[p''] inr ((p',g'),b',e',a') }}}. *)
-  (* Proof. *)
-  (*   iIntros (Hinstr Hfl Hfl' Hvpc Hpca' [Hwa Hwb] Hloc φ) *)
-  (*            "(>HPC & >Hi & >Hsrc & >Hdst & >Hsrca) Hφ". *)
-  (*   iDestruct (map_of_regs_3 with "HPC Hsrc Hdst") as "[Hmap (%&%&%)]". *)
-  (*   pose proof (writeAllowed_nonO _ _ Hfl' Hwa) as Hp''. *)
-  (*   pose proof (correctPC_nonO _ _ _ _ _ _ Hfl Hvpc) as Hpc_p'. *)
-  (*   iDestruct (memMap_resource_2ne_apply with "Hi Hsrca") as "[Hmem %]"; auto. *)
-
-  (*   iApply (wp_store _ pc_p with "[$Hmap $Hmem]"); eauto; simplify_map_eq; eauto. *)
-  (*   { by rewrite !dom_insert; set_solver+. } *)
-  (*   { eapply mem_neq_implies_allow_store_map with (a := a) (p' := p''); eauto. *)
-  (*     all: by simplify_map_eq. } *)
-  (*   iNext. iIntros (regs' mem' retv) "(#Hspec & Hmem & Hmap)". *)
-  (*   iDestruct "Hspec" as %Hspec. *)
-
-  (*   destruct Hspec as [ | * Hfail ]. *)
-  (*    { (* Success *) *)
-  (*      iApply "Hφ". *)
-  (*      destruct H7 as [Hrr2 _]. simplify_map_eq. *)
-  (*      rewrite insert_commute // insert_insert. *)
-  (*      iDestruct (memMap_resource_2ne with "Hmem") as "[Hpc_a Ha]";auto. *)
-  (*      incrementPC_inv. *)
-  (*      simplify_map_eq. *)
-  (*      rewrite insert_insert. *)
-  (*      iDestruct (regs_of_map_3 with "[$Hmap]") as "[HPC [Hsrc Hdst] ]"; eauto. iFrame. } *)
-  (*    { (* Failure (contradiction) *) *)
-  (*      destruct Hfail; try incrementPC_inv; simplify_map_eq; eauto. *)
-  (*      destruct o. all: try congruence. *)
-  (*      destruct Hloc as [_ Hpwl]. naive_solver. *)
-  (*    } *)
-  (* Qed. *)
-
-  (*  Lemma wp_store_success_z_reg E pc_p pc_g pc_b pc_e pc_a pc_a' w dst src w' *)
-  (*        p g b e a z pc_p' p' : *)
-  (*    decodeInstrW w = Store dst (inr src) → *)
-  (*    PermFlows pc_p pc_p' → *)
-  (*    PermFlows p p' → *)
-  (*    isCorrectPC (inr ((pc_p,pc_g),pc_b,pc_e,pc_a)) → *)
-  (*    (pc_a + 1)%a = Some pc_a' → *)
-  (*    writeAllowed p = true ∧ withinBounds ((p, g), b, e, a) = true → *)
-
-  (*    {{{ ▷ PC ↦ᵣ inr ((pc_p,pc_g),pc_b,pc_e,pc_a) *)
-  (*          ∗ ▷ pc_a ↦ₐ[pc_p'] w *)
-  (*          ∗ ▷ src ↦ᵣ inl z *)
-  (*          ∗ ▷ dst ↦ᵣ inr ((p,g),b,e,a) *)
-  (*          ∗ ▷ a ↦ₐ[p'] w' }}} *)
-  (*      Instr Executable @ E *)
-  (*      {{{ RET NextIV; *)
-  (*          PC ↦ᵣ inr ((pc_p,pc_g),pc_b,pc_e,pc_a') *)
-  (*             ∗ pc_a ↦ₐ[pc_p'] w *)
-  (*             ∗ src ↦ᵣ inl z *)
-  (*             ∗ dst ↦ᵣ inr ((p,g),b,e,a) *)
-  (*             ∗ a ↦ₐ[p'] inl z }}}. *)
-  (*  Proof. *)
-  (*    iIntros (Hinstr Hfl Hfl' Hvpc Hpca' [Hwa Hwb] φ) *)
-  (*            "(>HPC & >Hi & >Hsrc & >Hdst & >Hsrca) Hφ". *)
-  (*   iDestruct (map_of_regs_3 with "HPC Hsrc Hdst") as "[Hmap (%&%&%)]". *)
-  (*   pose proof (writeAllowed_nonO _ _ Hfl' Hwa) as Hp''. *)
-  (*   pose proof (correctPC_nonO _ _ _ _ _ _ Hfl Hvpc) as Hpc_p'. *)
-  (*   iDestruct (memMap_resource_2ne_apply with "Hi Hsrca") as "[Hmem %]"; auto. *)
-
-  (*   iApply (wp_store _ pc_p with "[$Hmap $Hmem]"); eauto; simplify_map_eq; eauto. *)
-  (*   { by rewrite !dom_insert; set_solver+. } *)
-  (*   { eapply mem_neq_implies_allow_store_map with (a := a) (p' := p'); eauto. *)
-  (*     all: by simplify_map_eq. } *)
-  (*   iNext. iIntros (regs' mem' retv) "(#Hspec & Hmem & Hmap)". *)
-  (*   iDestruct "Hspec" as %Hspec. *)
-
-  (*   destruct Hspec as [ | * Hfail ]. *)
-  (*    { (* Success *) *)
-  (*      iApply "Hφ". *)
-  (*      destruct H7 as [Hrr2 _]. simplify_map_eq. *)
-  (*      rewrite insert_commute // insert_insert. *)
-  (*      iDestruct (memMap_resource_2ne with "Hmem") as "[Hpc_a Ha]";auto. *)
-  (*      incrementPC_inv. *)
-  (*      simplify_map_eq. *)
-  (*      rewrite insert_insert. *)
-  (*      iDestruct (regs_of_map_3 with "[$Hmap]") as "[HPC [Hsrc Hdst] ]"; eauto. iFrame. } *)
-  (*    { (* Failure (contradiction) *) *)
-  (*      destruct Hfail; try incrementPC_inv; simplify_map_eq; eauto. *)
-  (*      destruct o. all: congruence. *)
-  (*    } *)
-  (*  Qed. *)
 
     Lemma wp_store_success_reg E pc_p pc_g pc_b pc_e pc_a pc_a' w dst src w'
          p g b e a w'' :
@@ -675,7 +387,6 @@ Section cap_lang_rules.
      (pc_a + 1)%a = Some pc_a' →
      writeAllowed p = true ∧ withinBounds ((p, g), b, e, a) = true →
      canStore p a w'' = true ->
-     (* (isLocalWord w'' = false ∨ (p = RWLX ∨ p = RWL)) → *)
 
      {{{ ▷ PC ↦ᵣ inr ((pc_p,pc_g),pc_b,pc_e,pc_a)
            ∗ ▷ pc_a ↦ₐ w
@@ -716,7 +427,7 @@ Section cap_lang_rules.
        destruct Hfail; try incrementPC_inv; simplify_map_eq; eauto.
        destruct o. all: try try congruence.
        destruct e0; try congruence.
-       inv Hvpc. destruct H6 as [? | [? | [? | [? | ?]]]]; destruct H13 as [? | [? | ?]]; congruence.
+       inv Hvpc. destruct H13 as [? | [? | ?]]; congruence.
      }
     Qed.
 
@@ -727,7 +438,6 @@ Section cap_lang_rules.
      (pc_a + 1)%a = Some pc_a' →
      writeAllowed p = true ∧ withinBounds ((p, g), b, e, a) = true →
      canStore p a (inr ((p,g),b,e,a)) = true ->
-     (* (isLocal g = false ∨ (p = RWLX ∨ p = RWL)) → *)
 
      {{{ ▷ PC ↦ᵣ inr ((pc_p,pc_g),pc_b,pc_e,pc_a)
            ∗ ▷ pc_a ↦ₐ w
@@ -766,7 +476,7 @@ Section cap_lang_rules.
        destruct Hfail; try incrementPC_inv; simplify_map_eq; eauto.
        destruct o. all: try congruence.
        destruct e0; try congruence.
-       inv Hvpc. destruct H4 as [? | [? | [? | [? | ?]]]]; destruct H11 as [? | [? | ?]]; congruence.
+       inv Hvpc.  destruct H11 as [? | [? | ?]]; congruence.
      }
     Qed.
 
@@ -814,7 +524,7 @@ Section cap_lang_rules.
        destruct Hfail; try incrementPC_inv; simplify_map_eq; eauto.
        destruct o. all: try congruence.
        destruct e0; try congruence.
-       inv Hvpc. destruct H4 as [? | [? | [? | [? | ?]]]]; destruct H11 as [? | [? | ?]]; congruence.
+       inv Hvpc. destruct H11 as [? | [? | ?]]; congruence.
      }
    Qed.
 
